Finished proof of confluence, thoughts on bisim restrictions

src/Concurrent/BisimReductions.v
@@ -1,1266 +1,6 @@
-From CoreErlang.Concurrent Require Import BarbedBisim.
+From CoreErlang.Concurrent Require Import BisimRenaming.
 
 Import ListNotations.
-
-Lemma ether_wf_rename :
-  forall eth p p',
-    ether_wf eth <-> ether_wf (renamePIDEther p p' eth).
-Proof.
-  split; intro; unfold ether_wf, renamePIDEther in *; intros.
-  * apply lookup_kmap_Some in H0. 2: auto. destruct H0 as [[s d] [Eq H0]].
-    simpl in Eq. inv Eq. rewrite lookup_fmap in H0.
-    destruct (eth !! (s, d)) eqn:P; setoid_rewrite P in H0. 2: inv H0.
-    apply H in P. inv H0.
-    apply Forall_forall. intros. rewrite Forall_forall in P.
-    apply in_map_iff in H0 as [? [? ?]]. apply P in H1.
-    subst x. now apply SIGCLOSED_rename.
-  * (* case separation needed for ι = p/p' *)
-    assert ((map (renamePIDSignal p p') <$> eth) !! (ι, ι') = map (renamePIDSignal p p') <$> Some l). {
-      rewrite lookup_fmap. by setoid_rewrite H0.
-    }
-    simpl in H1.
-    pose proof (lookup_kmap (prod_map (renamePIDPID_sym p p') (renamePIDPID_sym p p')) (map (renamePIDSignal p p') <$> eth) (ι, ι')).
-    setoid_rewrite <- H2 in H1. apply H in H1.
-    clear -H1. apply Basics.map_Forall in H1; auto.
-    intros. by apply SIGCLOSED_rename in H.
-Qed.
-
-Lemma spawnPIDs_subset_all :
-  forall l, list_to_set (PIDsOf spawnPIDOf l) ⊆ flat_union (fun '(a, ι) => {[ι]} ∪ usedPIDsAct a) l.
-Proof.
-  induction l; simpl; auto.
-  destruct a; simpl in *. case_match; simpl.
-  destruct a; inv H.
-  cbn. set_solver.
-  set_solver.
-Qed.
-
-Lemma sendPIDs_subset_all :
-  forall l, list_to_set (PIDsOf sendPIDOf l) ⊆ flat_union (fun '(a, ι) => {[ι]} ∪ usedPIDsAct a) l.
-Proof.
-  induction l; simpl; auto.
-  destruct a; simpl in *. case_match; simpl.
-  destruct a; inv H.
-  cbn. set_solver.
-  set_solver.
-Qed.
-
-Lemma rename_preCompatible:
-  forall O eth Π p p',
-  ¬isUsedPool p' Π ->
-  p' ∉ O ->
-  p ∉ O ->
-  preCompatibleNodes O (eth, Π)
-    (renamePIDEther p p' eth, renamePIDPool p p' Π).
-Proof.
-  split; simpl.
-  * apply lookup_kmap_None; auto. intros.
-    destruct H3. unfold renamePIDPID_sym in H4. repeat case_match; eqb_to_eq; subst.
-    - simpl in *. congruence.
-    - rewrite lookup_fmap.
-      assert (Π !! p' = None). {
-        apply eq_None_ne_Some_2. intros. intro. apply H. left.
-        intro. congruence.
-      }
-      now setoid_rewrite H4.
-    - rewrite lookup_fmap. simpl in *. now setoid_rewrite H3.
-  * destruct H3. simpl in *.
-    assert (ι ≠ p'). {
-      intro. subst. congruence.
-    }
-    assert (ι ≠ p). {
-      intro. subst.
-      congruence.
-    }
-    now apply isTargetedEther_rename_neq.
-Qed.
-
-Corollary rename_preCompatible_sym :
-  forall O eth Π p p',
-  ¬isUsedPool p' Π ->
-  p' ∉ O ->
-  p ∉ O ->
-  symClos (preCompatibleNodes O) (eth, Π)
-    (renamePIDEther p p' eth, renamePIDPool p p' Π).
-Proof.
-  intros. split.
-  * apply rename_preCompatible; auto.
-  * split; simpl.
-    - destruct H3. simpl in *. setoid_rewrite lookup_kmap_None in H3; auto.
-      specialize (H3 ι). unfold renamePIDPID_sym in H3.
-      repeat break_match_hyp; eqb_to_eq; subst.
-      + simpl in *. congruence.
-      + congruence.
-      + rewrite lookup_fmap in H3. simpl in *.
-        specialize (H3 eq_refl).
-        destruct (Π !! ι) eqn:P; setoid_rewrite P in H3. simpl in H3. congruence.
-        reflexivity.
-    - destruct H3. simpl in *.
-      assert (ι ≠ p'). {
-        intro. subst. congruence.
-      }
-      assert (ι ≠ p). {
-        intro. subst.
-        congruence.
-      }
-      by apply isTargetedEther_rename_neq in H4.
-Qed.
-
-(* This will not hold. For example, spawn + send to self won't be in the ether
-   or in the pool. *)
-Lemma impossible_send :
-  forall O n n' l, n -[l]ₙ->* n' with O ->
-    forall ι, ι ∈ (PIDsOf sendPIDOf l) ->
-      (isTargetedEther ι n.1 \/ isUsedPool ι n.2).
-Proof.
-  (* intros. induction H. inv H0.
-  unfold PIDsOf in H0. simpl in H0.
-  apply in_app_or in H0. destruct H0.
-  * destruct a; simpl in H0; inv H0. 2: contradiction.
-    inv H. 2: { clear -H2. intuition; congruence. }
-    simpl. right. right. exists ι0, p. split.
-    by setoid_rewrite lookup_insert. inv H7; simpl; auto.
-    - apply in_or_app. right. by left.
-    - apply in_or_app. right. by left.
-  * pose proof H0 as H0D. apply IHclosureNodeSem in H0. clear IHclosureNodeSem H1.
-    inv H;simpl in *.
-    - destruct H0.
-      + destruct (isUsedEther_dec ι ether). 1: by auto.
-        right. destruct (decide (ι = ι0)).
-        ** subst. left. by setoid_rewrite lookup_insert.
-        ** right. exists ι0, p.
-           split. by setoid_rewrite lookup_insert.
-           assert (ι = ι'). {
-             destruct H as [x0 [l0 H]]. unfold etherAdd in H.
-             unfold isUsedEther in H0.
-             assert (forall ιs l, ether !! (ιs, ι) <> Some l) by (clear -H0; firstorder).
-             case_match.
-             * destruct (decide ((ι0, ι') = (x0, ι))).
-               - inv e. by apply H2 in H3.
-               - setoid_rewrite lookup_insert_ne in H; auto.
-                 by apply H2 in H.
-             * destruct (decide ((ι0, ι') = (x0, ι))).
-               - inv e. reflexivity.
-               - setoid_rewrite lookup_insert_ne in H; auto.
-                 by apply H2 in H.
-           }
-           subst. inv H1; simpl; try by auto.
-           -- apply in_or_app. right. by left.
-           -- apply in_or_app. right. by left.
-      + apply isUsedPool_insert_1 in H. destruct_or!.
-        ** right. apply isUsedPool_insert_2. by left.
-        ** subst. right. left. by setoid_rewrite lookup_insert.
-        ** right.
-           clear H0D.
-           apply isUsedPool_insert_2. right. right.
-           inv H1; simpl in *. all: try right.
-           1-2,5: repeat (apply in_app_or in H as [|]); In_app_solver.
-           1-2: apply in_app_or in H as [|]; [In_app_solver |].
-           1: destruct H; subst; apply in_or_app; right; try by left.
-           1: right; repeat (apply in_app_or in H as [|]); In_app_solver.
-           repeat (apply in_app_or in H as [|]).
-           2-3: apply in_or_app; right; right; In_app_solver.
-           apply in_or_app; right. right. apply in_or_app.
-           left. apply in_remove in H; by apply H.
-    - destruct H0.
-      + left. eapply isUsedEther_etherPop_rev; eassumption.
-      + apply isUsedPool_insert_1 in H. destruct_or!.
-        ** right. apply isUsedPool_insert_2. by left.
-        ** subst. right. left. by setoid_rewrite lookup_insert.
-        ** inv H2; simpl in *.
-           all: repeat apply in_app_or in H as [|].
-           all: try by (right; apply isUsedPool_insert_2; right; right; In_app_solver).
-           -- rewrite flat_map_app in H. apply in_app_or in H as [|].
-              by (right; apply isUsedPool_insert_2; right; right; In_app_solver).
-              simpl in H. rewrite app_nil_r in H. *)
-Abort.
-
-
-Lemma fresh_pid_is_not_in_step :
-  forall O n n' a ι,
-  n -[ a | ι ]ₙ-> n' with O ->
-  (forall p',
-    ¬ isUsedPool p' n.2 ->
-    ¬ appearsEther p' n.1 ->
-    p' ∉ O ->
-   p' ∉ (usedPIDsAct a) \/ (exists v1 v2, a = ASpawn p' v1 v2 /\ p' ∉ usedPIDsVal v1 ∪ usedPIDsVal v2)).
-Proof.
-  intros. inv H; simpl in *. 1-3: left; intro.
-  * assert (p' = ι \/ (p' = ι' \/ p' ∈ usedPIDsSignal t)) by set_solver.
-    destruct H4.
-    - subst. apply H0. left. by setoid_rewrite lookup_insert.
-    - apply H0. clear -H3 H4.
-      right. exists ι, p. split. by setoid_rewrite lookup_insert.
-      inv H3; simpl in *; set_solver.
-  * destruct (decide (ι = p')).
-    - subst. apply H0. left. by setoid_rewrite lookup_insert.
-    - apply not_appearsEther_alt in H1. destruct_hyps.
-      unfold etherPop in H3. case_match. 2: congruence.
-      destruct l. 1: congruence.
-      inv H3. destruct (decide (p' = ι1)).
-      + subst. specialize (H5 ι). congruence.
-      + apply H6 in H7. simpl in H7. set_solver.
-  * destruct_or!; subst; simpl in *; try set_solver.
-    apply H0. left. assert (p' = ι) by set_solver. subst.
-    by setoid_rewrite lookup_insert.
-  * destruct (decide (ι' = p')).
-    - subst. right. do 2 eexists. split. reflexivity.
-      intro. apply H0. right. exists ι, p. split. by setoid_rewrite lookup_insert.
-      inv H8. set_solver.
-    - left. intro.
-      apply H0. right. exists ι, p. split. by setoid_rewrite lookup_insert.
-      inv H8; simpl in *.
-      clear-H n. set_solver.
-Qed.
-
-Theorem appearsEther_step :
-  forall O n n' a ι,
-  n -[ a | ι ]ₙ-> n' with O ->
-  forall ι',
-    ι' ∉ usedPIDsAct a ->
-    ¬appearsEther ι' n.1 ->
-    ¬appearsEther ι' n'.1.
-Proof.
-  intros. inv H; simpl in *; auto.
-  * intro. apply H1.
-    destruct H. 2: destruct H.
-    - left. apply isTargetedEther_etherAdd_rev in H; auto. intro. subst.
-      set_solver.
-    - destruct_hyps. unfold etherAdd in H. case_match.
-      + destruct (decide ((ι, ι'0) = (ι', x))).
-        ** inv e. setoid_rewrite lookup_insert in H.
-           right. left. exists x. by rewrite H3.
-        ** setoid_rewrite lookup_insert_ne in H; auto.
-           right. left. by exists x.
-      + destruct (decide ((ι, ι'0) = (ι', x))).
-        ** inv e. set_solver.
-        ** setoid_rewrite lookup_insert_ne in H; auto.
-           right. left. by exists x.
-    - destruct_hyps. unfold etherAdd. unfold etherAdd in H.
-      case_match.
-      + destruct (decide ((ι, ι'0) = (x, x0))).
-        ** inv e. setoid_rewrite lookup_insert in H. inv H.
-           right. right. exists x, x0, l.
-           split. assumption.
-           rewrite flat_union_app in H3. set_solver.
-        ** setoid_rewrite lookup_insert_ne in H; auto.
-           right. right. exists x, x0, x1.
-           split; assumption.
-      + destruct (decide ((ι, ι'0) = (x, x0))).
-        ** inv e. setoid_rewrite lookup_insert in H. inv H. set_solver.
-        ** setoid_rewrite lookup_insert_ne in H; auto.
-           right. right. exists x, x0, x1.
-           split; assumption.
-  * unfold etherPop in H2. case_match. 2: congruence.
-    case_match. 1: congruence.
-    inv H2. intro. apply H1. destruct H2. 2: destruct H2.
-    - left. destruct H2. destruct_hyps.
-      setoid_rewrite lookup_insert_ne in H2. 2: set_solver.
-      by exists x, x0.
-    - destruct_hyps. setoid_rewrite lookup_insert_ne in H2. 2: set_solver.
-      right. left. by exists x.
-    - destruct_hyps. destruct (decide ((ι1, ι) = (x, x0))).
-      + inv e. setoid_rewrite lookup_insert in H2. inv H2.
-        right. right. do 3 eexists. split. exact H.
-        simpl. set_solver.
-      + setoid_rewrite lookup_insert_ne in H2. 2: auto.
-        right. right. do 3 eexists. split; eassumption.
-Qed.
-
-Definition PIDRenamingList := list (PID * PID).
-Definition renamePIDs {A} (f : PID -> PID -> A -> A) (l : PIDRenamingList) (x : A) : A :=
-  fold_left (fun acc '(from, to) => f from to acc) l x.
-
-(*
-  If something is renamed, then it should not be renamed again
-  if the ith element of the list is (from, to) then from should not appear 
-
-*)
-(* P holds for l !! 0, o, then P holds for l !! 1, f (l !! 0) o, etc. *)
-Fixpoint collapse_list {A B : Set} (P : A -> B -> Prop) (f : A -> B -> B) (o : B) (l : list A) : Prop :=
-match l with
-| [] => True
-| x::xs => P x o /\ collapse_list P f (f x o) xs
-end.
-
-Definition PIDs_respect_node (O : gset PID) (n : Node) : list (PID * PID) -> Prop :=
-  collapse_list (fun '(from, to) n =>
-                   from ∉ O /\ to ∉ O /\ ¬isUsedPool to n.2 /\ ¬appearsEther to n.1)
-                (fun '(from, to) => prod_map (renamePIDEther from to) (renamePIDPool from to)) n.
-
-(* (* TODO: generalize this *)
-Fixpoint collapse_list (l : list (PID * PID)) (a : Action) :=
-match l with
-| (from, to)::l => to ∉ usedPIDsAct a /\ collapse_list l (renamePIDAct from to a)
-| [] => True
-end. *)
-
-Definition PIDs_respect_action (a : Action) : list (PID * PID) -> Prop :=
-  collapse_list (fun '(from, to) a => to ∉ usedPIDsAct a) (fun '(from, to) => renamePIDAct from to) a.
-
-Corollary renameList_preCompatible_sym :
-  forall O l eth Π,
-  PIDs_respect_node O (eth, Π) l ->
-  symClos (preCompatibleNodes O) (eth, Π)
-    (renamePIDs renamePIDEther l eth, renamePIDs renamePIDPool l Π).
-Proof.
-  induction l; intros.
-  cbn. split; apply preCompatibleNodes_refl.
-  inv H. destruct a. destruct_hyps. simpl in *.
-  split.
-  {
-    eapply preCompatibleNodes_trans.
-    eapply rename_preCompatible with (p := p) (p' := p0). 1-3: assumption.
-    apply IHl; try assumption.
-  }
-  {
-    eapply preCompatibleNodes_trans.
-    apply IHl; try assumption.
-    eapply rename_preCompatible_sym with (p := p) (p' := p0). 1-3: assumption.
-  }
-Qed.
-
-Corollary renameList_preCompatible_sym_old :
-  forall O l eth Π,
-  Forall (fun '(from, to) => ¬ isTargetedEther to eth /\ ¬isUsedPool to Π /\ to ∉ O /\ from ∉ O) l ->
-  NoDup (map snd l) ->
-  symClos (preCompatibleNodes O) (eth, Π)
-    (renamePIDs renamePIDEther l eth, renamePIDs renamePIDPool l Π).
-Proof.
-  induction l; intros.
-  cbn. split; apply preCompatibleNodes_refl.
-  inv H. destruct a. simpl.
-  split.
-  {
-    destruct_hyps. inv H0.
-    eapply preCompatibleNodes_trans.
-    eapply rename_preCompatible with (p := p) (p' := p0). 1-3: assumption.
-    apply IHl; try assumption.
-    {
-      clear -H H1 H4 H7 H8.
-      induction H4. constructor.
-      destruct x. inv H8. simpl in H7. destruct_hyps. constructor.
-      * split_and!; try assumption.
-        intro. apply isTargetedEther_rename_neq in H9. congruence. 2: set_solver.
-        intro. subst. apply isTargetedEther_rename_old in H9. congruence.
-        intro. apply isUsedPool_rename_neq in H9. congruence. 2: set_solver.
-        intro. subst. apply isUsedPool_rename_old in H9. congruence.
-      * apply IHForall; auto. (* set_solver. *)
-    }
-  }
-  {
-    destruct_hyps. inv H0.
-    eapply preCompatibleNodes_trans.
-    apply IHl; try assumption.
-    1: {
-      clear -H H1 H4 H7 H8.
-      induction H4; constructor; auto.
-      * destruct x.
-        clear IHForall. simpl in *.
-        destruct_and!. split_and!.
-        - intro. apply isTargetedEther_rename_neq in H5. congruence. 2: set_solver.
-          intro. subst. apply isTargetedEther_rename_old in H5. congruence.
-        - intro. apply isUsedPool_rename_neq in H5. congruence. 2: set_solver.
-          intro. subst. apply isUsedPool_rename_old in H5. congruence.
-        - set_solver.
-        - set_solver.
-      * apply IHForall; auto. set_solver. now inv H8.
-    }
-    eapply rename_preCompatible_sym with (p := p) (p' := p0). 1-3: assumption.
-  }
-Qed.
-
-
-Lemma ether_wf_renameList :
-  forall l eth,
-    ether_wf eth <-> ether_wf (renamePIDs renamePIDEther l eth).
-Proof.
-  induction l; intros.
-  * split; by simpl.
-  * split; simpl in *.
-    {
-      intro. destruct a.
-      apply -> IHl. by apply ether_wf_rename.
-    }
-    {
-      intro. destruct a.
-      apply IHl in H. by apply ether_wf_rename in H.
-    }
-Qed.
-
-Theorem renamePIDlist_is_preserved_node_semantics_1 :
-  forall l O eth eth' Π Π' a ι,
-    (eth, Π) -[a | ι]ₙ-> (eth', Π') with O ->
-      PIDs_respect_action a l ->
-      (* NoDup (map snd l) -> *)
-      PIDs_respect_node O (eth, Π) l ->
-      (renamePIDs renamePIDEther l eth, renamePIDs renamePIDPool l Π)
-    -[renamePIDs renamePIDAct l a | renamePIDs renamePIDPID_sym l ι]ₙ->
-      (renamePIDs renamePIDEther l eth', renamePIDs renamePIDPool l Π') with O.
-Proof.
-  induction l; intros. by assumption.
-  destruct a. simpl in *. inv H0. inv H1. destruct_hyps. simpl in *.
-  eapply IHl; auto.
-  {
-    apply renamePID_is_preserved_node_semantics; try assumption.
-  }
-Qed.
-
-Lemma PIDs_respect_node_preserved :
-  forall l O n n' a ι,
-    PIDs_respect_node O n l ->
-    PIDs_respect_action a l ->
-    n -[a | ι]ₙ-> n' with O ->
-    PIDs_respect_node O n' l.
-Proof.
-  induction l; intros. constructor. destruct n', n.
-  inv H. inv H0. destruct a. simpl in *. destruct_hyps. eapply IHl in H3; eauto.
-  2: { eapply renamePID_is_preserved_node_semantics. exact H1.
-       all: try assumption.
-     }
-  split.
-  * split_and!; auto. eapply not_isUsedPool_step; eauto.
-    eapply appearsEther_step in H1; eauto.
-  * exact H3.
-Qed.
-
-Lemma renamePIDPID_1 :
-  forall a b, renamePIDPID a b a = b.
-Proof.
-  unfold renamePIDPID. intros. by rewrite Nat.eqb_refl.
-Qed.
-
-Lemma renamePIDPID_sym_1 :
-  forall a b, renamePIDPID_sym a b a = b.
-Proof.
-  unfold renamePIDPID_sym. intros. by rewrite Nat.eqb_refl.
-Qed.
-
-Lemma PIDs_respect_action_take_drop :
-  forall l a,
-    (forall n, PIDs_respect_action (renamePIDs renamePIDAct (take n l) a) (drop n l)) ->
-    PIDs_respect_action a l.
-Proof.
-  induction l; intros. constructor.
-  split. destruct a.
-  * apply (H 0).
-  * destruct a. simpl. apply IHl. intros. apply (H (S n)).
-Qed.
-
-Fixpoint does_not_respect (l : list (PID * PID)) (a : Action) : gset PID :=
-match l with
-| [] => ∅
-| (from, to)::xs =>
-  if decide (to ∈ usedPIDsAct a)
-  then {[to]} ∪ (does_not_respect xs (renamePIDAct from to a) (* ∖ {[from]} *))
-  else does_not_respect xs (renamePIDAct from to a)  (* ∖ {[from]} *)
-end.
-
-Lemma PIDs_respect_node_respect_action_1 :
-  forall l a,
-    does_not_respect l a = ∅ ->
-    PIDs_respect_action a l.
-Proof.
-  induction l; intros. by constructor.
-    simpl in *. destruct a. inv H. destruct_hyps.
-    case_match.
-    - exfalso. set_solver.
-    - split. assumption.
-      by eapply IHl.
-Qed.
-
-Lemma does_not_respect_elem_of :
-  forall l from a, from ∈ does_not_respect l a ->
-    from ∈ map snd l.
-Proof.
-  induction l; intros. inv H.
-  simpl in *. destruct a. case_match.
-  * apply elem_of_union in H as [|].
-    - set_solver.
-    - simpl. apply IHl in H. set_solver.
-  * apply IHl in H. set_solver.
-Qed.
-
-Lemma PIDs_respect_node_elem_of_O :
-  forall l O n from,
-    PIDs_respect_node O n l ->
-    from ∈ map snd l ->
-    from ∉ O.
-Proof.
-  induction l; intros.
-  * set_solver.
-  * simpl in *. destruct a. inv H; simpl in *; destruct_hyps.
-    apply elem_of_cons in H0 as [|].
-    - subst. assumption.
-    - eapply IHl in H2; eassumption.
-Qed.
-
-Lemma fresh_PID_increases_respect :
-  forall l a from to ι,
-    to ∉ map snd l ->
-    to ∉ usedPIDsAct a ->
-    from ∉ map fst l ->
-    from ∉ map snd l ->
-    to ∉ map fst l ->
-    from ≠ to ->
-    ι ∈ does_not_respect l (renamePIDAct from to a) ->
-    ι ∈ does_not_respect l a ∖ {[from]}.
-Proof.
-  induction l; intros; simpl in *. set_solver.
-  destruct a.
-  rewrite usedPIDsAct_rename in H5; simpl in *.
-  repeat destruct decide.
-  * assert (p0 ≠ from) by set_solver.
-    destruct (decide (ι = p0)).
-    - set_solver.
-    - apply elem_of_union in H5 as [|]. 1: set_solver.
-      rewrite difference_union_distr_l_L. apply elem_of_union_r.
-      apply IHl with (to := to); auto. 1, 3-5: set_solver.
-      + rewrite usedPIDsAct_rename. destruct decide; set_solver.
-      + rewrite renamePID_swap_act. assumption.
-        ** intro. subst. set_solver.
-        ** lia.
-        ** set_solver.
-  * destruct (decide (ι = p0)).
-    - set_solver.
-    - apply elem_of_union in H5 as [|]. 1: set_solver.
-      apply IHl with (to := to); auto. 1, 3-5: set_solver.
-      + rewrite usedPIDsAct_rename. destruct decide; set_solver.
-      + rewrite renamePID_swap_act. assumption.
-        ** intro. subst. set_solver.
-        ** intro. set_solver.
-        ** set_solver.
-  * assert (p0 ≠ from) by set_solver.
-    destruct (decide (ι = p0)).
-    - set_solver.
-    - apply elem_of_union in H5 as [|]. 1: set_solver.
-      rewrite difference_union_distr_l_L. apply elem_of_union_r.
-      apply IHl with (to := to); auto. 1, 3-5: set_solver.
-      + rewrite usedPIDsAct_rename. destruct decide; set_solver.
-      + rewrite renamePID_swap_act. assumption.
-        ** intro. subst. set_solver.
-        ** lia.
-        ** set_solver.
-  * destruct (decide (ι = p0)).
-    - set_solver.
-    - apply elem_of_union in H5 as [|]. 1: set_solver.
-      apply IHl with (to := to); auto. 1, 3-5: set_solver.
-      + rewrite usedPIDsAct_rename. destruct decide; set_solver.
-      + rewrite renamePID_swap_act. assumption.
-        ** intro. subst. set_solver.
-        ** intro. set_solver.
-        ** set_solver.
-  * assert (to = p0) by set_solver. subst. set_solver.
-  * assert (to ≠ p0) by set_solver.
-    apply IHl with (to := to); auto. 1, 3-5: set_solver.
-    + rewrite usedPIDsAct_rename. destruct decide; set_solver.
-    + rewrite renamePID_swap_act. assumption.
-      ** intro. subst. set_solver.
-      ** intro. set_solver.
-      ** set_solver.
-  * assert (to = p0) by set_solver. subst. set_solver.
-  * assert (to ≠ p0) by set_solver.
-    apply IHl with (to := to); auto. 1, 3-5: set_solver.
-    + rewrite usedPIDsAct_rename. destruct decide; set_solver.
-    + rewrite renamePID_swap_act. assumption.
-      ** intro. subst. set_solver.
-      ** intro. set_solver.
-      ** set_solver.
-Qed.
-
-Lemma step_not_spawn_respects :
-  forall l a eth Π eth' Π' O ι,
-  (eth, Π) -[ a | ι ]ₙ-> (eth', Π') with O ->
-  PIDs_respect_node O (eth, Π) l ->
-  spawnPIDOf a = None -> does_not_respect l a = ∅.
-Proof.
-  induction l; intros.
-  * constructor.
-  * simpl in *. destruct a. inv H0. destruct_hyps.
-    case_match.
-    - simpl in *.
-      exfalso. inv H; simpl in *; try congruence.
-      + clear H6. destruct (decide (p0 = ι)).
-        ** apply H4. left. subst. setoid_rewrite lookup_insert. congruence.
-        ** apply H4. right.
-           exists ι, p1. split. by setoid_rewrite lookup_insert.
-           clear -e n H11. inv H11; simpl in *; set_solver.
-      + destruct (decide (p0 = ι)).
-        ** apply H4. left. subst. setoid_rewrite lookup_insert. congruence.
-        ** apply H5. unfold etherPop in H12.
-           do 2 (case_match; try congruence). inv H12.
-           right.
-           destruct (decide (p0 = ι1)).
-           -- subst. left. eexists. rewrite H. congruence.
-           -- right. do 3 eexists. split. exact H. simpl.
-              apply elem_of_union_l. clear -e n n0. set_solver.
-      + destruct_or!; subst; simpl in *.
-        ** set_solver.
-        ** apply H4. assert (p0 = ι) by (clear-e;set_solver).
-           subst. left. by setoid_rewrite lookup_insert.
-        ** clear-e. set_solver.
-        ** clear-e. set_solver.
-    - eapply IHl. 2: exact H3.
-      simpl. apply renamePID_is_preserved_node_semantics. exact H.
-      all: try assumption.
-      + clear -H1. destruct a0; auto. simpl in H1. congruence.
-Qed.
-
-Lemma fst_combine :
-  forall {A B} (l : list A) (l' : list B),
-    length l <= length l' ->
-    map fst (combine l l') = l.
-Proof.
-  induction l; destruct l'; simpl; intros.
-  1-2: reflexivity.
-  1: lia.
-  f_equal. apply IHl. lia.
-Qed.
-
-Lemma snd_combine :
-  forall {A B} (l : list A) (l' : list B),
-    length l' <= length l ->
-    map snd (combine l l') = l'.
-Proof.
-  induction l; destruct l'; simpl; intros.
-  1,3: reflexivity.
-  1: lia.
-  f_equal. apply IHl. lia.
-Qed.
-
-Definition allPIDsEther (eth : Ether) : gset PID :=
-  flat_union (fun '((ιs, ιd), sigs) => {[ιs; ιd]} ∪ flat_union usedPIDsSignal sigs) (map_to_list eth).
-Definition allPIDsPool (Π : ProcessPool) : gset PID :=
-  flat_union (fun '(ι, proc) => {[ι]} ∪ usedPIDsProc proc) (map_to_list Π).
-
-Lemma allPIDsPool_isNotUsed_1 :
-  forall ι Π,
-    ι ∉ allPIDsPool Π -> ¬isUsedPool ι Π.
-Proof.
-  intros. intro. destruct H0.
-  * apply H. apply elem_of_flat_union.
-    apply not_eq_None_Some in H0. destruct H0 as [proc H0].
-    exists (ι, proc). split. 2: set_solver.
-    by apply elem_of_map_to_list.
-  * apply H. apply elem_of_flat_union.
-    destruct H0 as [ι' [proc [P_1 P_2]]].
-    exists (ι', proc). split.
-    by apply elem_of_map_to_list.
-    set_solver.
-Qed.
-
-Lemma allPIDsPool_isNotUsed_2 :
-  forall ι Π,
-    ¬isUsedPool ι Π ->
-    ι ∉ allPIDsPool Π.
-Proof.
-  intros. intro. apply H.
-  unfold allPIDsPool in H0. apply elem_of_flat_union in H0.
-  destruct_hyps. destruct x as [ι' proc].
-  apply elem_of_map_to_list in H0 as P.
-  apply elem_of_union in H1 as [|].
-  * assert (ι = ι') by set_solver.
-    subst. left. by setoid_rewrite P.
-  * right. exists ι', proc. split; assumption.
-Qed.
-
-Lemma allPIDsEther_does_not_appear_1 :
-  forall ι eth,
-    ι ∉ allPIDsEther eth -> ¬appearsEther ι eth.
-Proof.
-  intros. intro. apply H.
-  apply elem_of_flat_union.
-  destruct H0. 2: destruct H0.
-  * destruct H0 as [ιs [l H0]].
-    exists (ιs, ι, l). split.
-    by apply elem_of_map_to_list.
-    set_solver.
-  * destruct H0 as [ιd H0].
-    apply not_eq_None_Some in H0. destruct H0 as [l H0].
-    exists (ι, ιd, l). split.
-    by apply elem_of_map_to_list.
-    set_solver.
-  * destruct H0 as [ιs [ιd [l [P1 P2]]]].
-    exists (ιs, ιd, l). split.
-    by apply elem_of_map_to_list.
-    set_solver.
-Qed.
-
-Lemma allPIDsEther_does_not_appear_2 :
-  forall ι eth,
-    ¬appearsEther ι eth ->
-    ι ∉ allPIDsEther eth.
-Proof.
-  intros. intro. apply H.
-  unfold allPIDsEther in H0. apply elem_of_flat_union in H0.
-  destruct_hyps. destruct x as [[ιs ιd] l].
-  apply elem_of_map_to_list in H0 as P.
-  apply elem_of_union in H1 as [|].
-  destruct (decide (ι = ιd)).
-  * subst. left. by exists ιs, l.
-  * assert (ι = ιs) by set_solver. subst. right. left.
-    exists ιd. by setoid_rewrite P.
-  * right. right. exists ιs, ιd, l. split; assumption.
-Qed.
-
-(** New idea: restrict semantics so that spawn cannot happen to appearing PIDs,
-   this way, the renaming does not do anything in this theorem! *)
-Lemma step_spawn_respects_3 :
-  forall l a eth Π eth' Π' O ι,
-  (eth, Π) -[ a | ι ]ₙ-> (eth', Π') with O ->
-  PIDs_respect_node O (eth, Π) l ->
-  forall p, spawnPIDOf a = Some p ->
-    exists new, new ∉ usedPIDsAct a /\ new ∉ O /\ ¬isUsedPool new Π /\ ¬appearsEther new eth /\ new ∉ map snd l /\
-    PIDs_respect_node O (eth, Π) ((p, new)::l) /\
-    PIDs_respect_action a ((p, new) :: l).
-Proof.
-  intros.
-  assert (exists new, new ∉ usedPIDsAct a /\ new ∉ O /\ ¬isUsedPool new Π /\ ¬appearsEther new eth /\ new ∉ map snd l /\ new ∉ map fst l). {
-    (* freshness *)
-    pose proof (infinite_is_fresh (elements (usedPIDsAct a) ++ elements O ++ elements (allPIDsPool Π) ++ elements (allPIDsEther eth) ++ map snd l ++ map fst l)).
-    remember (fresh _) as y in H2. clear-H2. exists y.
-    repeat apply not_elem_of_app in H2 as [? H2].
-    split_and!; try assumption.
-    1-2: set_solver.
-    * apply allPIDsPool_isNotUsed_1. set_solver.
-    * apply allPIDsEther_does_not_appear_1. set_solver.
-  }
-  destruct H2 as [new H2].
-  destruct_hyps. exists new. split_and!; try assumption.
-  * cbn. split_and!; try assumption.
-    1: {
-      destruct a; inv H1. inv H. destruct_or!; congruence.
-      assumption.
-    }
-    destruct a; inv H1. inv H. destruct_or!; congruence.
-    rewrite does_not_appear_renamePID_ether. 2-3: assumption.
-    rewrite isNotUsed_renamePID_pool. 2-3: assumption.
-    assumption.
-  * cbn. split; auto.
-    destruct a; inv H1. inv H. destruct_or!; congruence.
-    simpl.
-    assert (Ht1 : p ∉ usedPIDsVal t1). 2: assert (Ht2 : p ∉ usedPIDsVal t2).
-    1-2: intro; apply H17; right; exists ι, p0; setoid_rewrite lookup_insert; split; [reflexivity|].
-    1-2: inv H20; simpl; set_solver.
-    rewrite isNotUsed_renamePID_val. rewrite isNotUsed_renamePID_val.
-    2-3: assumption.
-    clear H19 H14.
-    renamePIDPID_case_match.
-    (* TODO: separate *)
-    {
-      clear -H6 H7 H0 H20.
-      assert (usedPIDsVal t1 ∪ usedPIDsVal t2 ⊆ usedPIDsProc p0). {
-        inv H20. set_solver.
-      }
-      clear H20.
-      generalize dependent l. intro l.
-      revert t1 t2 eth' ι p0 Π0 H. induction l; intros; cbn. trivial.
-      destruct a. simpl in *. inv H0. destruct_hyps.
-      split.
-      * intro. apply H3. right. exists ι, p0.
-        setoid_rewrite lookup_insert. split. reflexivity.
-        set_solver.
-      * renamePIDPID_case_match. 1: set_solver.
-        apply IHl with (p0 := renamePIDProc p1 p2 p0)
-                       (eth' := renamePIDEther p1 p2 eth')
-                       (Π0 := renamePIDPool p1 p2 Π0)
-                       (ι := renamePIDPID_sym p1 p2 ι).
-        + do 2 rewrite usedPIDsVal_rename.
-          rewrite usedPIDsProc_rename.
-          repeat destruct decide; set_solver.
-        + unfold PIDs_respect_node. cbn in H2.
-          setoid_rewrite <- kmap_insert; auto.
-          setoid_rewrite <- fmap_insert. exact H2.
-        + set_solver.
-        + set_solver.
-    }
-Qed.
-
-Definition swap {A B : Set} (a : A * B) : B * A := (a.2, a.1).
-
-Theorem cancel_renamePIDs_pool :
-  forall l O eth Π,
-  PIDs_respect_node O (eth, Π) l ->
-  renamePIDs renamePIDPool (map swap (reverse l)) (renamePIDs renamePIDPool l Π) = Π.
-Proof.
-  induction l; intros; simpl. reflexivity.
-  inv H. destruct a as [from to]. destruct_hyps. apply IHl in H1.
-  simpl in *.
-  rewrite reverse_cons, map_app. simpl.
-  unfold renamePIDs in *. rewrite fold_left_app. simpl.
-  rewrite H1.
-  by rewrite double_renamePID_pool.
-Qed.
-
-Theorem cancel_renamePIDs_ether :
-  forall l O eth Π,
-  PIDs_respect_node O (eth, Π) l ->
-  renamePIDs renamePIDEther (map swap (reverse l)) (renamePIDs renamePIDEther l eth) = eth.
-Proof.
-  induction l; intros; simpl. reflexivity.
-  inv H. destruct a as [from to]. destruct_hyps. apply IHl in H1.
-  simpl in *.
-  rewrite reverse_cons, map_app. simpl.
-  unfold renamePIDs in *. rewrite fold_left_app. simpl.
-  rewrite H1.
-  by rewrite double_renamePID_ether.
-Qed.
-
-Lemma PIDs_respect_node_app :
-  forall l₁ l₂ O n,
-    PIDs_respect_node O n (l₁ ++ l₂) <->
-    PIDs_respect_node O n l₁ /\
-    PIDs_respect_node O (prod_map (renamePIDs renamePIDEther l₁)
-                                  (renamePIDs renamePIDPool  l₁) n) l₂.
-Proof.
-  induction l₁; intros; cbn.
-  1: split; intros; destruct_hyps; try split; trivial; try assumption.
-  1-2: by destruct n.
-  destruct a. split; intros.
-  {
-    destruct_hyps. apply IHl₁ in H0 as [? ?]. split_and!; try assumption.
-  }
-  {
-    destruct_hyps. split_and!; try assumption.
-    apply IHl₁. split; assumption.
-  }
-Qed.
-
-Lemma cancel_PIDs_respect_node :
-  forall l O eth Π,
-  PIDs_respect_node O (eth, Π) l ->
-  PIDs_respect_node O (renamePIDs renamePIDEther l eth, renamePIDs renamePIDPool l Π)
-                      (map swap (reverse l)).
-Proof.
-  induction l; intros; simpl. constructor.
-  inv H. destruct a. simpl in *. apply IHl in H1 as H'. destruct_hyps.
-  rewrite reverse_cons, map_app. unfold swap at 2. cbn.
-  apply PIDs_respect_node_app. split. assumption.
-  cbn. split_and!; try assumption. 3: trivial.
-  * erewrite cancel_renamePIDs_pool. 2: exact H1.
-    intro. by apply isUsedPool_rename_old in H4.
-  * erewrite cancel_renamePIDs_ether. 2: exact H1.
-    intro. by apply appearsEther_rename_old in H4.
-Qed.
-
-(* TODO: this is not this simple:
-
-Theorem rename_bisim_alt :
-  forall O,
-    is_barbed_bisim_alt (
-      fun '(eth, Π) '(eth', Π') =>
-         forall l,
-          PIDs_respect_node O (eth, Π) l /\
-          renamePIDs renamePIDEther l eth = eth' /\
-          renamePIDs renamePIDPool l Π = Π'
-    ) O.
-Proof.
-  intros.
-  intros A B. destruct A as [eth Π]. destruct B.
-  intros. split_and!.
-  * intros. destruct A' as [eth' Π']. subst.
-    destruct (spawnPIDOf a) eqn:P.
-    { (* renaming needed *)
-      pose proof step_spawn_respects_3 l a _ _ _ _ _ _ H0 H _ P.
-      destruct H1 as [new H1]. destruct_hyps.
-      apply renamePIDlist_is_preserved_node_semantics_1 with (l := (p, new)::l) in H0 as D.
-      3: assumption.
-      2: assumption.
-
-      replace (renamePIDs renamePIDEther l eth) with
-         (renamePIDs renamePIDEther ((p, new) :: l) eth). 2: {
-         simpl.
-         rewrite does_not_appear_renamePID_ether; auto.
-         destruct a; inv P. inv H0. 1: destruct_or!; congruence.
-         by simpl.
-      }
-      replace (renamePIDs renamePIDPool l Π) with
-         (renamePIDs renamePIDPool ((p, new) :: l) Π). 2: {
-         simpl.
-         rewrite isNotUsed_renamePID_pool; auto.
-         destruct a; inv P. inv H0. 1: destruct_or!; congruence.
-         by simpl.
-      }
-      do 2 eexists. split. eapply n_trans. exact D. apply n_refl.
-      simpl. split_and!.
-      eapply PIDs_respect_node_preserved in H6; eassumption.
-    }
-    { (* renaming is not needed *)
-      eapply step_not_spawn_respects in H0 as R. 2: exact H. 2: assumption.
-      apply PIDs_respect_node_respect_action_1 in R as R'.
-      apply renamePIDlist_is_preserved_node_semantics_1 with (l := l) in H0 as D.
-      3: clear IH; assumption.
-      2: {
-        assumption.
-      }
-      do 2 eexists. split. eapply n_trans. exact D. apply n_refl.
-      apply IH; clear IH.
-      (* - eapply n_trans in H1. 2:apply n_refl.
-        by apply ether_wf_preserved in H1. *)
-      eapply PIDs_respect_node_preserved in H0; eassumption.
-    }
-  *
-  *
-  *
-Qed.  *)
-
-Unset Guard Checking.
-Theorem rename_bisim :
-  forall O eth Π (l : list (PID * PID)),
-    (* ether_wf eth -> *)
-    PIDs_respect_node O (eth, Π) l ->
-    (eth, Π) ~ (renamePIDs renamePIDEther l eth, renamePIDs renamePIDPool l Π) observing O.
-Proof.
-  cofix IH.
-  intros. constructor; auto.
-  (* * apply renameList_preCompatible_sym. assumption.
-  * simpl. by apply ether_wf_renameList. *)
-  * intros. destruct A' as [eth' Π'].
-    destruct (spawnPIDOf a) eqn:P.
-    { (* renaming needed *)
-      pose proof step_spawn_respects_3 l a _ _ _ _ _ _ H0 H _ P.
-      destruct H1 as [new H1]. destruct_hyps.
-      apply renamePIDlist_is_preserved_node_semantics_1 with (l := (p, new)::l) in H0 as D.
-      3: clear IH; assumption.
-      2: {
-        assumption.
-      }
-
-      replace (renamePIDs renamePIDEther l eth) with
-         (renamePIDs renamePIDEther ((p, new) :: l) eth). 2: {
-         simpl.
-         rewrite does_not_appear_renamePID_ether; auto.
-         destruct a; inv P. inv H0. 1: destruct_or!; congruence.
-         by simpl.
-      }
-      replace (renamePIDs renamePIDPool l Π) with
-         (renamePIDs renamePIDPool ((p, new) :: l) Π). 2: {
-         simpl.
-         rewrite isNotUsed_renamePID_pool; auto.
-         destruct a; inv P. inv H0. 1: destruct_or!; congruence.
-         by simpl.
-      }
-      do 2 eexists. split. eapply n_trans. exact D. apply n_refl.
-      apply IH; clear IH.
-(*       - eapply n_trans in H0. 2:apply n_refl.
-        by apply ether_wf_preserved in H0. *)
-      eapply PIDs_respect_node_preserved in H0; eassumption.
-    }
-    { (* renaming is not needed *)
-      eapply step_not_spawn_respects in H0 as R. 2: exact H. 2: assumption.
-      apply PIDs_respect_node_respect_action_1 in R as R'.
-      apply renamePIDlist_is_preserved_node_semantics_1 with (l := l) in H0 as D.
-      3: clear IH; assumption.
-      2: {
-        assumption.
-      }
-      do 2 eexists. split. eapply n_trans. exact D. apply n_refl.
-      apply IH; clear IH.
-      (* - eapply n_trans in H1. 2:apply n_refl.
-        by apply ether_wf_preserved in H1. *)
-      eapply PIDs_respect_node_preserved in H0; eassumption.
-    }
-  * clear IH.
-    simpl. intros.
-    exists (renamePIDs renamePIDPID_sym l source), []. eexists.
-    split.
-    {
-      apply n_refl.
-    }
-    {
-      simpl.
-      assert ((renamePIDs renamePIDPID_sym l source, dest) =
-           ((prod_map (renamePIDs renamePIDPID_sym l) (renamePIDs renamePIDPID_sym l)) (source, dest))). {
-        cbn. f_equal. clear -H H0.
-        generalize dependent dest. revert eth Π H.
-        induction l; intros. reflexivity.
-        inv H. destruct a. simpl.
-        intros. erewrite <- IHl; auto.
-        * unfold renamePIDPID_sym.
-          destruct_hyps. repeat case_match;eqb_to_eq; subst; try congruence.
-        * eassumption.
-        * unfold renamePIDPID_sym.
-          destruct_hyps. repeat case_match;eqb_to_eq; subst; try congruence.
-      }
-      setoid_rewrite H1.
-      {
-        clear. revert eth source dest.
-        induction l; intros; simpl.
-        * apply option_biforall_refl. intros. apply Signal_eq_refl.
-        * destruct a. eapply option_biforall_trans. 3: apply IHl.
-          - apply Signal_eq_trans.
-          - unfold renamePIDEther. replace (if source =? _ then _ else _, _) with
-              (prod_map (renamePIDPID_sym p p0) (renamePIDPID_sym p p0) (source, dest)) by reflexivity.
-            setoid_rewrite lookup_kmap; auto.
-            setoid_rewrite lookup_fmap.
-            simpl. destruct (eth !! _) eqn:P.
-            {
-              setoid_rewrite P. simpl.
-              eapply forall_biforall with (d1 := SUnlink) (d2 := SUnlink).
-              1: by rewrite map_length.
-              intros. rewrite map_nth with (d:= SUnlink).
-              by apply Signal_eq_renamePID.
-            }
-            {
-              setoid_rewrite P. simpl. trivial.
-            }
-      }
-    }
-  (* The other two cases need additional consideration. Now, it is allowed for l
-     to contain duplicates in its second elements.
-
-     Duplicates should be allowed in (map fst l), because we can't guarantee
-     that in the previous proof, the spawned PID "p" is not initially in
-     the (map fst l)
-     - Is this true? We could restrict l to contain only elements from the ether/pool
-     - But in the previous case, p cannot be added to l!
-
-     We can't do the proof by using double renaming, because it won't be guarded.
-     See the proof below, notice the use of "barbedBisim_sym"! : *)
-  * intros.
-    rewrite <- (cancel_renamePIDs_pool l O eth Π). 2: assumption.
-    rewrite <- (cancel_renamePIDs_ether l O eth Π). 2: assumption.
-
-    remember (map swap (reverse l)) as l'.
-    apply cancel_PIDs_respect_node in H as Hcancel.
-    rewrite <- Heql' in Hcancel.
-    destruct B' as [eth' Π'].
-    destruct (spawnPIDOf a) eqn:P.
-    { (* renaming needed *)
-      pose proof step_spawn_respects_3 l' a _ _ _ _ _ _ H0 Hcancel _ P.
-      destruct H1 as [new H1]. destruct_hyps.
-      apply renamePIDlist_is_preserved_node_semantics_1 with (l := (p, new)::l') in H0 as D.
-      3: clear IH; assumption.
-      2: {
-        assumption.
-      }
-
-      replace (renamePIDs renamePIDEther l' (renamePIDs renamePIDEther l eth)) with
-         (renamePIDs renamePIDEther ((p, new)::l') (renamePIDs renamePIDEther l eth)). 2: {
-         simpl.
-         rewrite does_not_appear_renamePID_ether; auto.
-         destruct a; inv P. inv H0. 1: destruct_or!; congruence.
-         by simpl.
-      }
-      replace (renamePIDs renamePIDPool l' (renamePIDs renamePIDPool l Π)) with
-         (renamePIDs renamePIDPool ((p, new) :: l') (renamePIDs renamePIDPool l Π)). 2: {
-         simpl.
-         rewrite isNotUsed_renamePID_pool; auto.
-         destruct a; inv P. inv H0. 1: destruct_or!; congruence.
-         by simpl.
-      }
-      do 2 eexists. split. eapply n_trans. exact D. apply n_refl.
-      (** NOTE: this use of symmetry makes the next use of IH unguarded *)
-      apply barbedBisim_sym.
-      apply IH; clear IH.
-      (** END NOTE *)
-      (* - eapply n_trans in H1. 2: apply n_refl.
-        apply ether_wf_preserved in H1. exact H1.
-        simpl. by apply ether_wf_renameList. *)
-      eapply PIDs_respect_node_preserved in H0; eassumption.
-    }
-    { (* renaming is not needed *)
-      eapply step_not_spawn_respects in H0 as R. 3: exact P. 2: exact Hcancel.
-      apply PIDs_respect_node_respect_action_1 in R as R'.
-      apply renamePIDlist_is_preserved_node_semantics_1 with (l := l') in H0 as D.
-      3: clear IH; assumption.
-      2: {
-        assumption.
-      }
-      do 2 eexists. split. eapply n_trans. exact D. apply n_refl.
-      (** NOTE: this use of symmetry makes the next use of IH unguarded *)
-      apply barbedBisim_sym.
-      apply IH; clear IH.
-      (** END NOTE *)
-(*       - eapply n_trans in H0. 2: apply n_refl.
-        apply ether_wf_preserved in H0. exact H.
-        simpl. by apply ether_wf_renameList. *)
-      - eapply PIDs_respect_node_preserved in H0; eassumption.
-    }
-  (* * intros. destruct B' as [eth' Π'].
-    destruct (spawnPIDOf a) eqn:P.
-    { (* renaming needed *)
-      (* pose proof step_spawn_respects_3 l a _ _ _ _ _ _ H1 H0 _ P.
-      destruct H2 as [new H2]. destruct_hyps.
-      apply renamePIDlist_is_preserved_node_semantics with (l := (p, new)::l) in H1 as D.
-      3: clear IH; assumption.
-      2: {
-        assumption.
-      }
-
-      replace (renamePIDs renamePIDEther l eth) with
-         (renamePIDs renamePIDEther ((p, new) :: l) eth). 2: {
-         simpl.
-         rewrite does_not_appear_renamePID_ether; auto.
-         destruct a; inv P. inv H1. 1: destruct_or!; congruence.
-         by simpl.
-      }
-      replace (renamePIDs renamePIDPool l Π) with
-         (renamePIDs renamePIDPool ((p, new) :: l) Π). 2: {
-         simpl.
-         rewrite isNotUsed_renamePID_pool; auto.
-         destruct a; inv P. inv H1. 1: destruct_or!; congruence.
-         by simpl.
-      }
-      do 2 eexists. split. eapply n_trans. exact D. apply n_refl.
-      apply IH; clear IH.
-      - eapply n_trans in H1. 2:apply n_refl.
-        by apply ether_wf_preserved in H1.
-      - eapply PIDs_respect_node_preserved in H1; eassumption. *)
-      admit.
-    }
-    { (* renaming is not needed *)
-      eapply step_not_spawn_respects in H1 as R. 3: exact P. 2: assumption.
-      apply PIDs_respect_node_respect_action_1 in R as R'.
-      apply renamePIDlist_is_preserved_node_semantics with (l := l) in H1 as D.
-      3: clear IH; assumption.
-      2: {
-        assumption.
-      }
-      do 2 eexists. split. eapply n_trans. exact D. apply n_refl.
-      apply IH; clear IH.
-      - eapply n_trans in H1. 2:apply n_refl.
-        by apply ether_wf_preserved in H1.
-      - eapply PIDs_respect_node_preserved in H1; eassumption.
-    } *)
-  * clear IH. intros. simpl.
-    assert (exists source', option_list_biforall Signal_eq
-      (renamePIDs renamePIDEther l eth !! (source, dest))
-      (eth !! (source', dest))). {
-      revert l eth Π source H0 H. induction l; intros.
-      * inv H0. simpl. exists source.
-        apply option_biforall_refl. intros.
-        apply Signal_eq_refl.
-      * simpl. destruct a. inv H. cbn in H1. apply IHl with (source := source) in H2.
-        2: assumption.
-        destruct_hyps.
-        simpl in *.
-        destruct (decide (x = p)). 2: destruct (decide (x = p0)).
-        (* TODO: shorten, these 3 cases are almost the same. The difference
-           is the variables need to be used: x vs p vs p0. *)
-        {
-          subst. replace (p, dest) with (prod_map (renamePIDPID_sym p p0) (renamePIDPID_sym p p0) (p0, dest)) in H.
-          2: {
-            cbn. renamePIDPID_sym_case_match; try reflexivity;congruence.
-          }
-          setoid_rewrite lookup_kmap in H; auto.
-          setoid_rewrite lookup_fmap in H.
-          exists p0.
-          eapply option_biforall_trans. 1: apply Signal_eq_trans.
-          exact H.
-          simpl. destruct (eth !! _) eqn:P.
-          {
-            setoid_rewrite P. simpl.
-            eapply forall_biforall with (d1 := SUnlink) (d2 := SUnlink).
-            1: by rewrite map_length.
-            intros. rewrite map_nth with (d:= SUnlink).
-            pose proof (Signal_eq_renamePID (nth i l0 SUnlink) p p0).
-            unfold Signal_eq in *.
-            rewrite <- H6.
-            by rewrite Signal_eq_sym, Signal_eq_renamePID.
-          }
-          {
-            setoid_rewrite P. simpl. trivial.
-          }
-        }
-        {
-          subst. replace (p0, dest) with (prod_map (renamePIDPID_sym p p0) (renamePIDPID_sym p p0) (p, dest)) in H.
-          2: {
-            cbn. renamePIDPID_sym_case_match; try reflexivity;congruence.
-          }
-          setoid_rewrite lookup_kmap in H; auto.
-          setoid_rewrite lookup_fmap in H.
-          exists p.
-          eapply option_biforall_trans. 1: apply Signal_eq_trans.
-          exact H.
-          simpl. destruct (eth !! _) eqn:P.
-          {
-            setoid_rewrite P. simpl.
-            eapply forall_biforall with (d1 := SUnlink) (d2 := SUnlink).
-            1: by rewrite map_length.
-            intros. rewrite map_nth with (d:= SUnlink).
-            pose proof (Signal_eq_renamePID (nth i l0 SUnlink) p p0).
-            unfold Signal_eq in *.
-            rewrite <- H6.
-            by rewrite Signal_eq_sym, Signal_eq_renamePID.
-          }
-          {
-            setoid_rewrite P. simpl. trivial.
-          }
-        }
-        {
-          subst. replace (x, dest) with (prod_map (renamePIDPID_sym p p0) (renamePIDPID_sym p p0) (x, dest)) in H.
-          2: {
-            cbn. renamePIDPID_sym_case_match; try reflexivity;congruence.
-          }
-          setoid_rewrite lookup_kmap in H; auto.
-          setoid_rewrite lookup_fmap in H.
-          exists x.
-          eapply option_biforall_trans. 1: apply Signal_eq_trans.
-          exact H.
-          simpl. destruct (eth !! _) eqn:P.
-          {
-            setoid_rewrite P. simpl.
-            eapply forall_biforall with (d1 := SUnlink) (d2 := SUnlink).
-            1: by rewrite map_length.
-            intros. rewrite map_nth with (d:= SUnlink).
-            pose proof (Signal_eq_renamePID (nth i l0 SUnlink) p p0).
-            unfold Signal_eq in *.
-            rewrite <- H6.
-            by rewrite Signal_eq_sym, Signal_eq_renamePID.
-          }
-          {
-            setoid_rewrite P. simpl. trivial.
-          }
-        }
-    }
-    destruct H1. exists x, []. eexists.
-    split. apply n_refl.
-    assumption.
-Defined.
-Set Guard Checking.
-
-Lemma reductions_preserve_O_dom :
-  forall l O n n', n -[l]ₙ->* n' with O ->
-    O ## dom n.2 ->
-    O ## dom n'.2.
-Proof.
-  induction l; intros; inv H. assumption.
-  apply IHl in H6. assumption.
-  clear IHl H6. inv H4; simpl in *; setoid_rewrite dom_insert; setoid_rewrite dom_insert in H0; try assumption.
-  clear H5. setoid_rewrite dom_insert. set_solver.
-Qed.
-
-Lemma reductions_preserve_singals_targeting_O :
-  forall O (n n' : Node) l, n -[l]ₙ->* n' with O ->
-    O ## dom n.2 ->
-    (forall ι, ι ∈ (PIDsOf sendPIDOf l) -> ι ∉ O) ->
-    forall source : PID,
-      (* n'.2 !! dest = None -> *)
-      forall dest, dest ∈ O ->
-      option_list_biforall Signal_eq (n.1 !! (source, dest)) (n'.1 !! (source, dest)).
-Proof.
-  intros O n n' l H. induction H; intros Hdom H1 ? ? Hin.
-  1: apply option_biforall_refl; intros; apply Signal_eq_refl.
-  eapply option_biforall_trans.
-    1: by apply Signal_eq_trans.
-    2: apply IHclosureNodeSem. 3-4: set_solver.
-    2: eapply reductions_preserve_O_dom; [|eassumption].
-    2: eapply n_trans; [ exact H | apply n_refl ].
-  inversion H; subst; simpl in *.
-  3-4: apply option_biforall_refl; intros; apply Signal_eq_refl.
-  * unfold etherAdd. destruct (decide ((ι, ι') = (source, dest))).
-    - inv e. case_match; exfalso; apply H1 in Hin; try assumption; set_solver.
-    - break_match_goal; setoid_rewrite lookup_insert_ne; try assumption; auto.
-      all: apply option_biforall_refl; intros; apply Signal_eq_refl.
-  * unfold etherPop in H2. destruct (decide ((ι1, ι) = (source, dest))).
-    - inv e.
-      case_match. 2: congruence. destruct l0; try congruence. inv H2.
-      exfalso. clear -Hin Hdom. set_solver.
-    - case_match; try congruence. destruct l0; try congruence. inv H2.
-      setoid_rewrite lookup_insert_ne; auto.
-      apply option_biforall_refl; intros; apply Signal_eq_refl.
-Qed.
 
 Theorem action_options :
   forall O n n' n'' a ι a' ι',
@@ -1312,6 +52,8 @@ Proof.
     all: try (inv H7; by cbn in *).
     all: try (inv H8; by cbn in *).
     all: try (inv H; by cbn in *).
+    congruence.
+    congruence.
   (* spawn + local - PIDs should be different *)
   * subst. put (lookup ι' : ProcessPool -> option Process) on H3 as P.
     setoid_rewrite lookup_insert in P. inv P.
@@ -1466,9 +208,10 @@ Proof.
   all: apply Val_eq_dec.
 Defined.
 
+(* Arrive and ε actions create non-confluent reductions with any other reduction of the same process instrumented by the inter-process semantics. *)
 Definition isChainable (a : Action) : Prop :=
 match a with
- | AArrive _ _ _ | ASetFlag => False
+ | AArrive _ _ _ | ε | ASend _ _ SLink | ASend _ _ SUnlink => False
  | _ => True
 end.
 
@@ -1646,6 +389,58 @@ TODO: this cases a lot of boiler plate
              }
              setoid_rewrite H0.
              eapply n_other. by constructor. by left.
+      (* recv_peek_message - success *)
+      + eexists. split.
+        1: { constructor. eassumption. constructor. }
+        right.
+        assert (ι
+ ↦ inl
+     (FParams (IPrimOp "recv_peek_message") [] [] :: fs0, RBox,
+      mailboxPush mb v, links, flag) ∥ prs = ι
+ ↦ inl
+     (FParams (IPrimOp "recv_peek_message") [] [] :: fs0, RBox,
+      mailboxPush mb v, links, flag) ∥ Π). {
+               apply map_eq. intros.
+               clear -H1.
+               put (lookup i : ProcessPool -> _) on H1 as HH.
+               destruct (decide (i = ι)).
+               * subst. by setoid_rewrite lookup_insert.
+               * setoid_rewrite lookup_insert_ne; auto.
+                 setoid_rewrite lookup_insert_ne in HH; auto.
+             }
+             setoid_rewrite H0.
+             eapply n_other. eapply p_recv_peek_message_ok.
+             { destruct mb; clear-H10. simpl.
+               destruct l0; inv H10. reflexivity. }
+             by left.
+      (* removeMessage *)
+      + eexists. split.
+        1: { constructor. eassumption. constructor. }
+        right.
+        assert (ι
+ ↦ inl
+     (FParams (IPrimOp "remove_message") [] [] :: fs0, RBox,
+      mailboxPush mb v, links, flag) ∥ prs = ι
+ ↦ inl
+     (FParams (IPrimOp "remove_message") [] [] :: fs0, RBox,
+      mailboxPush mb v, links, flag) ∥ Π). {
+          apply map_eq. intros.
+          clear -H1.
+          put (lookup i : ProcessPool -> _) on H1 as HH.
+          destruct (decide (i = ι)).
+          * subst. by setoid_rewrite lookup_insert.
+          * setoid_rewrite lookup_insert_ne; auto.
+            setoid_rewrite lookup_insert_ne in HH; auto.
+        }
+        setoid_rewrite H0.
+        eapply n_other.
+        econstructor.
+        {
+          clear -H10. destruct mb. simpl in *.
+          destruct l0; invSome. simpl.
+          by rewrite app_assoc.
+        }
+        by left.
       (* recv_wait_timeout 0 *)
       + eexists. split.
         1: { constructor. eassumption. constructor. }
@@ -1709,116 +504,17 @@ TODO: this cases a lot of boiler plate
              }
              setoid_rewrite H0.
              eapply n_other. by constructor. by right; left.
-      (* recv_peek_message - success *)
-      + eexists. split.
-        1: { constructor. eassumption. constructor. }
-        right.
-        assert (ι
- ↦ inl
-     (FParams (IPrimOp "recv_peek_message") [] [] :: fs0, RBox,
-      mailboxPush mb v, links, flag) ∥ prs = ι
- ↦ inl
-     (FParams (IPrimOp "recv_peek_message") [] [] :: fs0, RBox,
-      mailboxPush mb v, links, flag) ∥ Π). {
-               apply map_eq. intros.
-               clear -H1.
-               put (lookup i : ProcessPool -> _) on H1 as HH.
-               destruct (decide (i = ι)).
-               * subst. by setoid_rewrite lookup_insert.
-               * setoid_rewrite lookup_insert_ne; auto.
-                 setoid_rewrite lookup_insert_ne in HH; auto.
-             }
-             setoid_rewrite H0.
-             eapply n_other. econstructor.
-             { destruct mb; clear-H10. simpl.
-               destruct l0; inv H10. reflexivity. }
-             by right; right; left.
       (* recv_peek_message - fail - This cannot be proved
          after pushing a message, peekMessage won't fail anymore *)
-      + admit.
+      + inv H.
       (* recv_next *)
-      + eexists. split.
-        1: { constructor. eassumption. constructor. }
-        right.
-        assert (ι
- ↦ inl
-     (FParams (IPrimOp "recv_next") [] [] :: fs0, RBox, 
-      mailboxPush mb v, links, flag) ∥ prs = ι
- ↦ inl
-     (FParams (IPrimOp "recv_next") [] [] :: fs0, RBox, 
-      mailboxPush mb v, links, flag) ∥ Π). {
-           apply map_eq. intros.
-           clear -H1.
-           put (lookup i : ProcessPool -> _) on H1 as HH.
-           destruct (decide (i = ι)).
-           * subst. by setoid_rewrite lookup_insert.
-           * setoid_rewrite lookup_insert_ne; auto.
-             setoid_rewrite lookup_insert_ne in HH; auto.
-         }
-         setoid_rewrite H0.
-         destruct mb as [old new]. destruct new.
-         1: admit. (* This won't work if the mailbox is empty *)
-         assert (mailboxPush (recvNext (old, v0 :: new)) v = recvNext (mailboxPush (old, v0 :: new) v)) by reflexivity.
-         rewrite H2.
-         eapply n_other. econstructor.
-         by right; right; left.
-      (* removeMessage *)
-      + eexists. split.
-        1: { constructor. eassumption. constructor. }
-        right.
-        assert (ι
- ↦ inl
-     (FParams (IPrimOp "remove_message") [] [] :: fs0, RBox,
-      mailboxPush mb v, links, flag) ∥ prs = ι
- ↦ inl
-     (FParams (IPrimOp "remove_message") [] [] :: fs0, RBox,
-      mailboxPush mb v, links, flag) ∥ Π). {
-          apply map_eq. intros.
-          clear -H1.
-          put (lookup i : ProcessPool -> _) on H1 as HH.
-          destruct (decide (i = ι)).
-          * subst. by setoid_rewrite lookup_insert.
-          * setoid_rewrite lookup_insert_ne; auto.
-            setoid_rewrite lookup_insert_ne in HH; auto.
-        }
-        setoid_rewrite H0.
-        eapply n_other.
-        econstructor.
-        {
-          clear -H10. destruct mb. simpl in *.
-          destruct l0; invSome. simpl.
-          by rewrite app_assoc.
-        }
-        by right; right; left.
+      + inv H.
       (* recv_wait_timeout infinity *)
-      + eexists. split.
-        1: { constructor. eassumption. constructor. }
-        right.
-        assert (ι
- ↦ inl
-     (FParams (IPrimOp "recv_wait_timeout") [] [] :: fs0,
-      RValSeq [VLit "infinity"%string], mailboxPush (oldmb, msg :: newmb) v, links,
-      flag) ∥ prs = ι
- ↦ inl
-     (FParams (IPrimOp "recv_wait_timeout") [] [] :: fs0,
-      RValSeq [VLit "infinity"%string], mailboxPush (oldmb, msg :: newmb) v, links,
-      flag) ∥ Π). {
-               apply map_eq. intros.
-               clear -H1.
-               put (lookup i : ProcessPool -> _) on H1 as HH.
-               destruct (decide (i = ι)).
-               * subst. by setoid_rewrite lookup_insert.
-               * setoid_rewrite lookup_insert_ne; auto.
-                 setoid_rewrite lookup_insert_ne in HH; auto.
-             }
-        setoid_rewrite H0.
-        eapply n_other.
-        econstructor.
-        by right; right; left.
+      + inv H.
       (* normal termination *)
-      + admit. (* arrive can't be chained on a dead process *)
+      + inv H. (* arrive can't be chained on a dead process *)
       (* exceptional termination *)
-      + admit. (* arrive can't be chained on a dead process *)
+      + inv H. (* arrive can't be chained on a dead process *)
       (* setflag *)
       + inv H.
     (* spawn *)
@@ -1891,7 +587,7 @@ TODO: this cases a lot of boiler plate
         right.
         eapply n_send. by constructor.
       (* link send *)
-      + admit. (* can't be done *)
+      + inv H. (* can't be done *)
       (* unlink send *)
       + eexists. split.
         1: { constructor. apply etherPop_greater. eassumption.
@@ -1917,6 +613,14 @@ TODO: this cases a lot of boiler plate
       + eexists. split.
         1: { constructor. eassumption. constructor. assumption. }
         right. eapply n_other. by constructor. by left.
+      (* recv_peek_message - success *)
+      + eexists. split.
+        1: { constructor. eassumption. constructor. assumption. }
+        right. eapply n_other. by constructor. by left.
+      (* removeMessage *)
+      + eexists. split.
+        1: { constructor. eassumption. constructor. assumption. }
+        right. eapply n_other. by constructor. by intuition.
       (* recv_wait_timeout 0 *)
       + eexists. split.
         1: { constructor. eassumption. constructor. assumption. }
@@ -1929,10 +633,6 @@ TODO: this cases a lot of boiler plate
       + eexists. split.
         1: { constructor. eassumption. constructor. assumption. }
         right. eapply n_other. by constructor. by right;left.
-      (* recv_peek_message - success *)
-      + eexists. split.
-        1: { constructor. eassumption. constructor. assumption. }
-        right. eapply n_other. by constructor. by right;right;left.
       (* recv_peek_message - fail *)
       + eexists. split.
         1: { constructor. eassumption. constructor. assumption. }
@@ -1941,18 +641,14 @@ TODO: this cases a lot of boiler plate
       + eexists. split.
         1: { constructor. eassumption. constructor. assumption. }
         right. eapply n_other. by constructor. by intuition.
-      (* removeMessage *)
-      + eexists. split.
-        1: { constructor. eassumption. constructor. assumption. }
-        right. eapply n_other. by constructor. by intuition.
       (* recv_wait_timeout infinity *)
       + eexists. split.
         1: { constructor. eassumption. constructor. assumption. }
         right. eapply n_other. by constructor. by intuition.
       (* normal termination *)
-      + admit. (* arrive can't be chained on a dead process *)
+      + inv H. (* arrive can't be chained on a dead process *)
       (* exceptional termination *)
-      + admit. (* arrive can't be chained on a dead process *)
+      + inv H. (* arrive can't be chained on a dead process *)
       (* setflag *)
       + inv H.
     (* spawn *)
@@ -2008,9 +704,9 @@ TODO: this cases a lot of boiler plate
         put (lookup i : ProcessPool -> _) on H2 as H'.
         by setoid_rewrite lookup_insert_ne in H'.
       (* link send - can't be done, since links are potentially modified *)
-      + admit.
+      + inv H.
       (* unlink send - can't be done, since links are potentially modified *)
-      + admit.
+      + inv H.
     (* arrivals - cannot happen *)
     - inv H.
     (* local actions *)
@@ -2024,6 +720,30 @@ TODO: this cases a lot of boiler plate
 *)
       destruct_or! H9; subst; inv H2.
       (* silent steps *)
+      + eexists. split.
+        1: { constructor. eassumption.
+             apply p_exit_terminate. set_solver.
+           }
+        left. simpl. eexists. split. 1: eassumption.
+        f_equal. apply map_eq.
+        intros. destruct (decide (ι = i)).
+        1: subst; by setoid_rewrite lookup_insert.
+        setoid_rewrite lookup_insert_ne; auto.
+        put (lookup i : ProcessPool -> _) on H1 as H'.
+        by setoid_rewrite lookup_insert_ne in H'.
+      (* recv_peek_message - success *)
+      + eexists. split.
+        1: { constructor. eassumption.
+             apply p_exit_terminate. set_solver.
+           }
+        left. simpl. eexists. split. 1: eassumption.
+        f_equal. apply map_eq.
+        intros. destruct (decide (ι = i)).
+        1: subst; by setoid_rewrite lookup_insert.
+        setoid_rewrite lookup_insert_ne; auto.
+        put (lookup i : ProcessPool -> _) on H1 as H'.
+        by setoid_rewrite lookup_insert_ne in H'.
+      (* removeMessage *)
       + eexists. split.
         1: { constructor. eassumption.
              apply p_exit_terminate. set_solver.
@@ -2071,18 +791,6 @@ TODO: this cases a lot of boiler plate
         setoid_rewrite lookup_insert_ne; auto.
         put (lookup i : ProcessPool -> _) on H1 as H'.
         by setoid_rewrite lookup_insert_ne in H'.
-      (* recv_peek_message - success *)
-      + eexists. split.
-        1: { constructor. eassumption.
-             apply p_exit_terminate. set_solver.
-           }
-        left. simpl. eexists. split. 1: eassumption.
-        f_equal. apply map_eq.
-        intros. destruct (decide (ι = i)).
-        1: subst; by setoid_rewrite lookup_insert.
-        setoid_rewrite lookup_insert_ne; auto.
-        put (lookup i : ProcessPool -> _) on H1 as H'.
-        by setoid_rewrite lookup_insert_ne in H'.
       (* recv_peek_message - fail *)
       + eexists. split.
         1: { constructor. eassumption.
@@ -2107,18 +815,6 @@ TODO: this cases a lot of boiler plate
         setoid_rewrite lookup_insert_ne; auto.
         put (lookup i : ProcessPool -> _) on H1 as H'.
         by setoid_rewrite lookup_insert_ne in H'.
-      (* removeMessage *)
-      + eexists. split.
-        1: { constructor. eassumption.
-             apply p_exit_terminate. set_solver.
-           }
-        left. simpl. eexists. split. 1: eassumption.
-        f_equal. apply map_eq.
-        intros. destruct (decide (ι = i)).
-        1: subst; by setoid_rewrite lookup_insert.
-        setoid_rewrite lookup_insert_ne; auto.
-        put (lookup i : ProcessPool -> _) on H1 as H'.
-        by setoid_rewrite lookup_insert_ne in H'.
       (* recv_wait_timeout infinity *)
       + eexists. split.
         1: { constructor. eassumption.
@@ -2132,9 +828,9 @@ TODO: this cases a lot of boiler plate
         put (lookup i : ProcessPool -> _) on H1 as H'.
         by setoid_rewrite lookup_insert_ne in H'.
       (* normal termination *)
-      + admit. (* arrive can't be chained on a dead process *)
+      + inv H. (* arrive can't be chained on a dead process *)
       (* exceptional termination *)
-      + admit. (* arrive can't be chained on a dead process *)
+      + inv H. (* arrive can't be chained on a dead process *)
       (* setflag *)
       + inv H.
     (* spawn -
@@ -2192,16 +888,16 @@ TODO: this cases a lot of boiler plate
       :: fs0, RValSeq [v],
       mailboxPush mb (VTuple [VLit "EXIT"%string; VPid ιs; reason]), links,
       true) ∥ prs0). {
-               apply map_eq. intros.
-               clear -H2.
-               put (lookup i : ProcessPool -> _) on H2 as HH.
-               destruct (decide (i = ι)).
-               * subst. by setoid_rewrite lookup_insert.
-               * setoid_rewrite lookup_insert_ne; auto.
-                 setoid_rewrite lookup_insert_ne in HH; auto.
-             }
-             setoid_rewrite H0.
-             eapply n_send. by constructor.
+          apply map_eq. intros.
+          clear -H2.
+          put (lookup i : ProcessPool -> _) on H2 as HH.
+          destruct (decide (i = ι)).
+          * subst. by setoid_rewrite lookup_insert.
+          * setoid_rewrite lookup_insert_ne; auto.
+            setoid_rewrite lookup_insert_ne in HH; auto.
+        }
+        setoid_rewrite H0.
+        eapply n_send. by constructor.
       (* exit send *)
       + eexists. split.
         1: { constructor. apply etherPop_greater. eassumption.
@@ -2219,16 +915,16 @@ TODO: this cases a lot of boiler plate
         VPid ι'] [] :: fs0, RValSeq [v],
       mailboxPush mb (VTuple [VLit "EXIT"%string; VPid ιs; reason]), links,
       true) ∥ prs0). {
-               apply map_eq. intros.
-               clear -H2.
-               put (lookup i : ProcessPool -> _) on H2 as HH.
-               destruct (decide (i = ι)).
-               * subst. by setoid_rewrite lookup_insert.
-               * setoid_rewrite lookup_insert_ne; auto.
-                 setoid_rewrite lookup_insert_ne in HH; auto.
-             }
-             setoid_rewrite H0.
-             eapply n_send. by constructor.
+          apply map_eq. intros.
+          clear -H2.
+          put (lookup i : ProcessPool -> _) on H2 as HH.
+          destruct (decide (i = ι)).
+          * subst. by setoid_rewrite lookup_insert.
+          * setoid_rewrite lookup_insert_ne; auto.
+            setoid_rewrite lookup_insert_ne in HH; auto.
+        }
+        setoid_rewrite H0.
+        eapply n_send. by constructor.
       (* link send - maybe this should not be proved? *)
       + eexists. split.
         1: { constructor. apply etherPop_greater. eassumption.
@@ -2248,18 +944,18 @@ TODO: this cases a lot of boiler plate
       :: fs0, RValSeq [VPid ι'],
       mailboxPush mb (VTuple [VLit "EXIT"%string; VPid ιs; reason]), links,
       true) ∥ prs0). {
-               apply map_eq. intros.
-               clear -H2.
-               put (lookup i : ProcessPool -> _) on H2 as HH.
-               destruct (decide (i = ι)).
-               * subst. by setoid_rewrite lookup_insert.
-               * setoid_rewrite lookup_insert_ne; auto.
-                 setoid_rewrite lookup_insert_ne in HH; auto.
-             }
-             setoid_rewrite H0.
-             eapply n_send. by constructor.
+        apply map_eq. intros.
+        clear -H2.
+        put (lookup i : ProcessPool -> _) on H2 as HH.
+        destruct (decide (i = ι)).
+        * subst. by setoid_rewrite lookup_insert.
+        * setoid_rewrite lookup_insert_ne; auto.
+          setoid_rewrite lookup_insert_ne in HH; auto.
+      }
+      setoid_rewrite H0.
+      eapply n_send. by constructor.
       (* unlink send - can't be proved, list of links influence the behaviour of exits *)
-      + admit.
+      + inv H.
     (* arrivals - cannot happen *)
     - inv H.
     (* local actions *)
@@ -2283,89 +979,16 @@ TODO: this cases a lot of boiler plate
  ↦ inl
      (fs, e, mailboxPush mb (VTuple [VLit "EXIT"%string; VPid ιs; reason]),
       links, true) ∥ Π). {
-               apply map_eq. intros.
-               clear -H1.
-               put (lookup i : ProcessPool -> _) on H1 as HH.
-               destruct (decide (i = ι)).
-               * subst. by setoid_rewrite lookup_insert.
-               * setoid_rewrite lookup_insert_ne; auto.
-                 setoid_rewrite lookup_insert_ne in HH; auto.
-             }
-             setoid_rewrite H0.
-             eapply n_other. by constructor. by left.
-      (* recv_wait_timeout 0 *)
-      + eexists. split.
-        1: { constructor. eassumption. by apply p_exit_convert. }
-        right.
-        assert (ι
- ↦ inl
-     (FParams (IPrimOp "recv_wait_timeout") [] [] :: fs0, RValSeq [
-      VLit 0%Z],
-      mailboxPush mb (VTuple [VLit "EXIT"%string; VPid ιs; reason]), links,
-      true) ∥ prs = ι
- ↦ inl
-     (FParams (IPrimOp "recv_wait_timeout") [] [] :: fs0, RValSeq [
-      VLit 0%Z],
-      mailboxPush mb (VTuple [VLit "EXIT"%string; VPid ιs; reason]), links,
-      true) ∥ Π). {
-               apply map_eq. intros.
-               clear -H1.
-               put (lookup i : ProcessPool -> _) on H1 as HH.
-               destruct (decide (i = ι)).
-               * subst. by setoid_rewrite lookup_insert.
-               * setoid_rewrite lookup_insert_ne; auto.
-                 setoid_rewrite lookup_insert_ne in HH; auto.
-             }
-             setoid_rewrite H0.
-             eapply n_other. by constructor. by left.
-      (* recv_wait_timeout error *)
-      + eexists. split.
-        1: { constructor. eassumption. by apply p_exit_convert. }
-        right.
-        assert (ι
- ↦ inl
-     (FParams (IPrimOp "recv_wait_timeout") [] [] :: fs0, RValSeq [v],
-      mailboxPush mb (VTuple [VLit "EXIT"%string; VPid ιs; reason]), links,
-      true) ∥ prs = ι
- ↦ inl
-     (FParams (IPrimOp "recv_wait_timeout") [] [] :: fs0, RValSeq [v],
-      mailboxPush mb (VTuple [VLit "EXIT"%string; VPid ιs; reason]), links,
-      true) ∥ Π). {
-               apply map_eq. intros.
-               clear -H1.
-               put (lookup i : ProcessPool -> _) on H1 as HH.
-               destruct (decide (i = ι)).
-               * subst. by setoid_rewrite lookup_insert.
-               * setoid_rewrite lookup_insert_ne; auto.
-                 setoid_rewrite lookup_insert_ne in HH; auto.
-             }
-             setoid_rewrite H0.
-             eapply n_other. by constructor. by left.
-      (* self *)
-      + eexists. split.
-        1: { constructor. eassumption. by apply p_exit_convert. }
-        right.
-        assert (ι
- ↦ inl
-     (FParams (ICall (VLit "erlang"%string) (VLit "self"%string)) [] []
-      :: fs0, RBox,
-      mailboxPush mb (VTuple [VLit "EXIT"%string; VPid ιs; reason]), links,
-      true) ∥ prs = ι
- ↦ inl
-     (FParams (ICall (VLit "erlang"%string) (VLit "self"%string)) [] []
-      :: fs0, RBox,
-      mailboxPush mb (VTuple [VLit "EXIT"%string; VPid ιs; reason]), links,
-      true) ∥ Π). {
-               apply map_eq. intros.
-               clear -H1.
-               put (lookup i : ProcessPool -> _) on H1 as HH.
-               destruct (decide (i = ι)).
-               * subst. by setoid_rewrite lookup_insert.
-               * setoid_rewrite lookup_insert_ne; auto.
-                 setoid_rewrite lookup_insert_ne in HH; auto.
-             }
-             setoid_rewrite H0.
-             eapply n_other. by constructor. by right; left.
+          apply map_eq. intros.
+          clear -H1.
+          put (lookup i : ProcessPool -> _) on H1 as HH.
+          destruct (decide (i = ι)).
+          * subst. by setoid_rewrite lookup_insert.
+          * setoid_rewrite lookup_insert_ne; auto.
+            setoid_rewrite lookup_insert_ne in HH; auto.
+        }
+        setoid_rewrite H0.
+        eapply n_other. by constructor. by left.
       (* recv_peek_message - success *)
       + eexists. split.
         1: { constructor. eassumption. by apply p_exit_convert. }
@@ -2379,50 +1002,19 @@ TODO: this cases a lot of boiler plate
      (FParams (IPrimOp "recv_peek_message") [] [] :: fs0, RBox,
       mailboxPush mb (VTuple [VLit "EXIT"%string; VPid ιs; reason]), links,
       true) ∥ Π). {
-               apply map_eq. intros.
-               clear -H1.
-               put (lookup i : ProcessPool -> _) on H1 as HH.
-               destruct (decide (i = ι)).
-               * subst. by setoid_rewrite lookup_insert.
-               * setoid_rewrite lookup_insert_ne; auto.
-                 setoid_rewrite lookup_insert_ne in HH; auto.
-             }
-             setoid_rewrite H0.
-             eapply n_other. econstructor.
-             { destruct mb; clear-H11. simpl.
-               destruct l0; inv H11. reflexivity. }
-             by right; right; left.
-      (* recv_peek_message - fail - This cannot be proved
-         after pushing a message, peekMessage won't fail anymore *)
-      + admit.
-      (* recv_next *)
-      + eexists. split.
-        1: { constructor. eassumption. by apply p_exit_convert. }
-        right.
-        assert (ι
- ↦ inl
-     (FParams (IPrimOp "recv_next") [] [] :: fs0, RBox,
-      mailboxPush mb (VTuple [VLit "EXIT"%string; VPid ιs; reason]), links,
-      true) ∥ prs = ι
- ↦ inl
-     (FParams (IPrimOp "recv_next") [] [] :: fs0, RBox,
-      mailboxPush mb (VTuple [VLit "EXIT"%string; VPid ιs; reason]), links,
-      true) ∥ Π). {
-           apply map_eq. intros.
-           clear -H1.
-           put (lookup i : ProcessPool -> _) on H1 as HH.
-           destruct (decide (i = ι)).
-           * subst. by setoid_rewrite lookup_insert.
-           * setoid_rewrite lookup_insert_ne; auto.
-             setoid_rewrite lookup_insert_ne in HH; auto.
-         }
-         setoid_rewrite H0.
-         destruct mb as [old new]. destruct new.
-         1: admit. (* This won't work if the mailbox is empty *)
-         assert (mailboxPush (recvNext (old, v :: new)) (VTuple [VLit "EXIT"%string; VPid ιs; reason]) = recvNext (mailboxPush (old, v :: new) (VTuple [VLit "EXIT"%string; VPid ιs; reason]))) by reflexivity.
-         rewrite H2.
-         eapply n_other. econstructor.
-         by right; right; left.
+          apply map_eq. intros.
+          clear -H1.
+          put (lookup i : ProcessPool -> _) on H1 as HH.
+          destruct (decide (i = ι)).
+          * subst. by setoid_rewrite lookup_insert.
+          * setoid_rewrite lookup_insert_ne; auto.
+            setoid_rewrite lookup_insert_ne in HH; auto.
+        }
+        setoid_rewrite H0.
+        eapply n_other. eapply p_recv_peek_message_ok.
+        { destruct mb; clear-H11. simpl.
+          destruct l0; inv H11. reflexivity. }
+        by left.
       (* removeMessage *)
       + eexists. split.
         1: { constructor. eassumption. by apply p_exit_convert. }
@@ -2452,7 +1044,111 @@ TODO: this cases a lot of boiler plate
          destruct l0; invSome. simpl.
          by rewrite app_assoc.
        }
-       by right; right; left.
+       by intuition.
+      (* recv_wait_timeout 0 *)
+      + eexists. split.
+        1: { constructor. eassumption. by apply p_exit_convert. }
+        right.
+        assert (ι
+ ↦ inl
+     (FParams (IPrimOp "recv_wait_timeout") [] [] :: fs0, RValSeq [
+      VLit 0%Z],
+      mailboxPush mb (VTuple [VLit "EXIT"%string; VPid ιs; reason]), links,
+      true) ∥ prs = ι
+ ↦ inl
+     (FParams (IPrimOp "recv_wait_timeout") [] [] :: fs0, RValSeq [
+      VLit 0%Z],
+      mailboxPush mb (VTuple [VLit "EXIT"%string; VPid ιs; reason]), links,
+      true) ∥ Π). {
+          apply map_eq. intros.
+          clear -H1.
+          put (lookup i : ProcessPool -> _) on H1 as HH.
+          destruct (decide (i = ι)).
+          * subst. by setoid_rewrite lookup_insert.
+          * setoid_rewrite lookup_insert_ne; auto.
+            setoid_rewrite lookup_insert_ne in HH; auto.
+        }
+        setoid_rewrite H0.
+        eapply n_other. by constructor. by left.
+      (* recv_wait_timeout error *)
+      + eexists. split.
+        1: { constructor. eassumption. by apply p_exit_convert. }
+        right.
+        assert (ι
+ ↦ inl
+     (FParams (IPrimOp "recv_wait_timeout") [] [] :: fs0, RValSeq [v],
+      mailboxPush mb (VTuple [VLit "EXIT"%string; VPid ιs; reason]), links,
+      true) ∥ prs = ι
+ ↦ inl
+     (FParams (IPrimOp "recv_wait_timeout") [] [] :: fs0, RValSeq [v],
+      mailboxPush mb (VTuple [VLit "EXIT"%string; VPid ιs; reason]), links,
+      true) ∥ Π). {
+          apply map_eq. intros.
+          clear -H1.
+          put (lookup i : ProcessPool -> _) on H1 as HH.
+          destruct (decide (i = ι)).
+          * subst. by setoid_rewrite lookup_insert.
+          * setoid_rewrite lookup_insert_ne; auto.
+            setoid_rewrite lookup_insert_ne in HH; auto.
+        }
+        setoid_rewrite H0.
+        eapply n_other. by constructor. by left.
+      (* self *)
+      + eexists. split.
+        1: { constructor. eassumption. by apply p_exit_convert. }
+        right.
+        assert (ι
+ ↦ inl
+     (FParams (ICall (VLit "erlang"%string) (VLit "self"%string)) [] []
+      :: fs0, RBox,
+      mailboxPush mb (VTuple [VLit "EXIT"%string; VPid ιs; reason]), links,
+      true) ∥ prs = ι
+ ↦ inl
+     (FParams (ICall (VLit "erlang"%string) (VLit "self"%string)) [] []
+      :: fs0, RBox,
+      mailboxPush mb (VTuple [VLit "EXIT"%string; VPid ιs; reason]), links,
+      true) ∥ Π). {
+          apply map_eq. intros.
+          clear -H1.
+          put (lookup i : ProcessPool -> _) on H1 as HH.
+          destruct (decide (i = ι)).
+          * subst. by setoid_rewrite lookup_insert.
+          * setoid_rewrite lookup_insert_ne; auto.
+            setoid_rewrite lookup_insert_ne in HH; auto.
+        }
+        setoid_rewrite H0.
+        eapply n_other. by constructor. by right; left.
+      (* recv_peek_message - fail - This cannot be proved
+         after pushing a message, peekMessage won't fail anymore *)
+      + inv H.
+      (* recv_next *)
+      + inv H. (* eexists. split.
+        1: { constructor. eassumption. by apply p_exit_convert. }
+        right.
+        assert (ι
+ ↦ inl
+     (FParams (IPrimOp "recv_next") [] [] :: fs0, RBox,
+      mailboxPush mb (VTuple [VLit "EXIT"%string; VPid ιs; reason]), links,
+      true) ∥ prs = ι
+ ↦ inl
+     (FParams (IPrimOp "recv_next") [] [] :: fs0, RBox,
+      mailboxPush mb (VTuple [VLit "EXIT"%string; VPid ιs; reason]), links,
+      true) ∥ Π). {
+           apply map_eq. intros.
+           clear -H1.
+           put (lookup i : ProcessPool -> _) on H1 as HH.
+           destruct (decide (i = ι)).
+           * subst. by setoid_rewrite lookup_insert.
+           * setoid_rewrite lookup_insert_ne; auto.
+             setoid_rewrite lookup_insert_ne in HH; auto.
+         }
+         setoid_rewrite H0.
+         destruct mb as [old new]. destruct new.
+         1: admit. (* This won't work if the mailbox is empty *)
+         assert (mailboxPush (recvNext (old, v :: new)) (VTuple [VLit "EXIT"%string; VPid ιs; reason]) = recvNext (mailboxPush (old, v :: new) (VTuple [VLit "EXIT"%string; VPid ιs; reason]))) by reflexivity.
+         rewrite H2.
+         eapply n_other. econstructor.
+         by intuition. *)
       (* recv_wait_timeout infinity *)
       + eexists. split.
         1: { constructor. eassumption. by apply p_exit_convert. }
@@ -2479,11 +1175,11 @@ TODO: this cases a lot of boiler plate
         setoid_rewrite H0.
         eapply n_other.
         econstructor.
-        by right; right; left.
+        by intuition.
       (* normal termination *)
-      + admit. (* arrive can't be chained on a dead process *)
+      + inv H. (* arrive can't be chained on a dead process *)
       (* exceptional termination *)
-      + admit. (* arrive can't be chained on a dead process *)
+      + inv H. (* arrive can't be chained on a dead process *)
       (* setflag *)
       + inv H.
     (* spawn *)
@@ -2568,16 +1264,16 @@ TODO: this cases a lot of boiler plate
  ↦ inl
      (FParams (ICall (VLit "erlang"%string) (VLit "!"%string)) [VPid ι'] []
       :: fs0, RValSeq [v], mb, ιs :: links, flag) ∥ prs0). {
-               apply map_eq. intros.
-               clear -H2.
-               put (lookup i : ProcessPool -> _) on H2 as HH.
-               destruct (decide (i = ι)).
-               * subst. by setoid_rewrite lookup_insert.
-               * setoid_rewrite lookup_insert_ne; auto.
-                 setoid_rewrite lookup_insert_ne in HH; auto.
-             }
-             setoid_rewrite H0.
-             eapply n_send. by constructor.
+          apply map_eq. intros.
+          clear -H2.
+          put (lookup i : ProcessPool -> _) on H2 as HH.
+          destruct (decide (i = ι)).
+          * subst. by setoid_rewrite lookup_insert.
+          * setoid_rewrite lookup_insert_ne; auto.
+            setoid_rewrite lookup_insert_ne in HH; auto.
+        }
+        setoid_rewrite H0.
+        eapply n_send. by constructor.
       (* exit send *)
       + eexists. split.
         1: { constructor. apply etherPop_greater. eassumption.
@@ -2591,16 +1287,16 @@ TODO: this cases a lot of boiler plate
  ↦ inl
      (FParams (ICall (VLit "erlang"%string) (VLit "exit"%string)) [
         VPid ι'] [] :: fs0, RValSeq [v], mb, ιs :: links, flag) ∥ prs0). {
-               apply map_eq. intros.
-               clear -H2.
-               put (lookup i : ProcessPool -> _) on H2 as HH.
-               destruct (decide (i = ι)).
-               * subst. by setoid_rewrite lookup_insert.
-               * setoid_rewrite lookup_insert_ne; auto.
-                 setoid_rewrite lookup_insert_ne in HH; auto.
-             }
-             setoid_rewrite H0.
-             eapply n_send. by constructor.
+          apply map_eq. intros.
+          clear -H2.
+          put (lookup i : ProcessPool -> _) on H2 as HH.
+          destruct (decide (i = ι)).
+          * subst. by setoid_rewrite lookup_insert.
+          * setoid_rewrite lookup_insert_ne; auto.
+            setoid_rewrite lookup_insert_ne in HH; auto.
+        }
+        setoid_rewrite H0.
+        eapply n_send. by constructor.
       (* link send - maybe this should not be proved? *)
       + eexists. split.
         1: { constructor. apply etherPop_greater. eassumption.
@@ -2614,18 +1310,18 @@ TODO: this cases a lot of boiler plate
  ↦ inl
      (FParams (ICall (VLit "erlang"%string) (VLit "link"%string)) [] []
       :: fs0, RValSeq [VPid ι'], mb, ιs :: links, flag) ∥ prs0). {
-               apply map_eq. intros.
-               clear -H2.
-               put (lookup i : ProcessPool -> _) on H2 as HH.
-               destruct (decide (i = ι)).
-               * subst. by setoid_rewrite lookup_insert.
-               * setoid_rewrite lookup_insert_ne; auto.
-                 setoid_rewrite lookup_insert_ne in HH; auto.
-             }
-             setoid_rewrite H0.
-             eapply n_send. admit. (* TODO: links should be formalised as sets *)
+          apply map_eq. intros.
+          clear -H2.
+          put (lookup i : ProcessPool -> _) on H2 as HH.
+          destruct (decide (i = ι)).
+          * subst. by setoid_rewrite lookup_insert.
+          * setoid_rewrite lookup_insert_ne; auto.
+            setoid_rewrite lookup_insert_ne in HH; auto.
+        }
+        setoid_rewrite H0.
+        eapply n_send. inv H. (* TODO: links should be formalised as sets *)
       (* unlink send - can't be proved if the same link is established and deleted in the two reductions *)
-      + admit.
+      + inv H.
     (* arrivals - cannot happen *)
     - inv H.
     (* local actions *)
@@ -2643,79 +1339,16 @@ TODO: this cases a lot of boiler plate
         1: { constructor. eassumption. constructor. }
         right.
         assert (ι ↦ inl (fs, e, mb, ιs :: links, flag) ∥ prs = ι ↦ inl (fs, e, mb, ιs :: links, flag) ∥ Π). {
-               apply map_eq. intros.
-               clear -H1.
-               put (lookup i : ProcessPool -> _) on H1 as HH.
-               destruct (decide (i = ι)).
-               * subst. by setoid_rewrite lookup_insert.
-               * setoid_rewrite lookup_insert_ne; auto.
-                 setoid_rewrite lookup_insert_ne in HH; auto.
-             }
-             setoid_rewrite H0.
-             eapply n_other. by constructor. by left.
-      (* recv_wait_timeout 0 *)
-      + eexists. split.
-        1: { constructor. eassumption. constructor. }
-        right.
-        assert (ι
- ↦ inl
-     (FParams (IPrimOp "recv_wait_timeout") [] [] :: fs0, RValSeq [
-      VLit 0%Z], mb, ιs :: links, flag) ∥ prs = ι
- ↦ inl
-     (FParams (IPrimOp "recv_wait_timeout") [] [] :: fs0, RValSeq [
-      VLit 0%Z], mb, ιs :: links, flag) ∥ Π). {
-               apply map_eq. intros.
-               clear -H1.
-               put (lookup i : ProcessPool -> _) on H1 as HH.
-               destruct (decide (i = ι)).
-               * subst. by setoid_rewrite lookup_insert.
-               * setoid_rewrite lookup_insert_ne; auto.
-                 setoid_rewrite lookup_insert_ne in HH; auto.
-             }
-             setoid_rewrite H0.
-             eapply n_other. by constructor. by left.
-      (* recv_wait_timeout error *)
-      + eexists. split.
-        1: { constructor. eassumption. constructor. }
-        right.
-        assert (ι
- ↦ inl
-     (FParams (IPrimOp "recv_wait_timeout") [] [] :: fs0, RValSeq [v], mb,
-      ιs :: links, flag) ∥ prs = ι
- ↦ inl
-     (FParams (IPrimOp "recv_wait_timeout") [] [] :: fs0, RValSeq [v], mb,
-      ιs :: links, flag) ∥ Π). {
-               apply map_eq. intros.
-               clear -H1.
-               put (lookup i : ProcessPool -> _) on H1 as HH.
-               destruct (decide (i = ι)).
-               * subst. by setoid_rewrite lookup_insert.
-               * setoid_rewrite lookup_insert_ne; auto.
-                 setoid_rewrite lookup_insert_ne in HH; auto.
-             }
-             setoid_rewrite H0.
-             eapply n_other. by constructor. by left.
-      (* self *)
-      + eexists. split.
-        1: { constructor. eassumption. constructor. }
-        right.
-        assert (ι
- ↦ inl
-     (FParams (ICall (VLit "erlang"%string) (VLit "self"%string)) [] []
-      :: fs0, RBox, mb, ιs :: links, flag) ∥ prs = ι
- ↦ inl
-     (FParams (ICall (VLit "erlang"%string) (VLit "self"%string)) [] []
-      :: fs0, RBox, mb, ιs :: links, flag) ∥ Π). {
-               apply map_eq. intros.
-               clear -H1.
-               put (lookup i : ProcessPool -> _) on H1 as HH.
-               destruct (decide (i = ι)).
-               * subst. by setoid_rewrite lookup_insert.
-               * setoid_rewrite lookup_insert_ne; auto.
-                 setoid_rewrite lookup_insert_ne in HH; auto.
-             }
-             setoid_rewrite H0.
-             eapply n_other. by constructor. by right; left.
+          apply map_eq. intros.
+          clear -H1.
+          put (lookup i : ProcessPool -> _) on H1 as HH.
+          destruct (decide (i = ι)).
+          * subst. by setoid_rewrite lookup_insert.
+          * setoid_rewrite lookup_insert_ne; auto.
+            setoid_rewrite lookup_insert_ne in HH; auto.
+        }
+        setoid_rewrite H0.
+        eapply n_other. by constructor. by left.
       (* recv_peek_message - success *)
       + eexists. split.
         1: { constructor. eassumption. constructor. }
@@ -2727,63 +1360,18 @@ TODO: this cases a lot of boiler plate
  ↦ inl
      (FParams (IPrimOp "recv_peek_message") [] [] :: fs0, RBox, mb,
       ιs :: links, flag) ∥ Π). {
-               apply map_eq. intros.
-               clear -H1.
-               put (lookup i : ProcessPool -> _) on H1 as HH.
-               destruct (decide (i = ι)).
-               * subst. by setoid_rewrite lookup_insert.
-               * setoid_rewrite lookup_insert_ne; auto.
-                 setoid_rewrite lookup_insert_ne in HH; auto.
-             }
-             setoid_rewrite H0.
-             eapply n_other. econstructor.
-             assumption.
-             by right; right; left.
-      (* recv_peek_message - fail *)
-      + eexists. split.
-        1: { constructor. eassumption. constructor. }
-        right.
-        assert (ι
- ↦ inl
-     (FParams (IPrimOp "recv_peek_message") [] [] :: fs0, RBox, mb,
-      ιs :: links, flag) ∥ prs = ι
- ↦ inl
-     (FParams (IPrimOp "recv_peek_message") [] [] :: fs0, RBox, mb,
-      ιs :: links, flag) ∥ Π). {
-               apply map_eq. intros.
-               clear -H1.
-               put (lookup i : ProcessPool -> _) on H1 as HH.
-               destruct (decide (i = ι)).
-               * subst. by setoid_rewrite lookup_insert.
-               * setoid_rewrite lookup_insert_ne; auto.
-                 setoid_rewrite lookup_insert_ne in HH; auto.
-             }
-             setoid_rewrite H0.
-             eapply n_other. econstructor.
-             assumption.
-             by right; right; left.
-      (* recv_next *)
-      + eexists. split.
-        1: { constructor. eassumption. constructor. }
-        right.
-        assert (ι
- ↦ inl
-     (FParams (IPrimOp "recv_next") [] [] :: fs0, RBox, mb, 
-      ιs :: links, flag) ∥ prs = ι
- ↦ inl
-     (FParams (IPrimOp "recv_next") [] [] :: fs0, RBox, mb, 
-      ιs :: links, flag) ∥ Π). {
-           apply map_eq. intros.
-           clear -H1.
-           put (lookup i : ProcessPool -> _) on H1 as HH.
-           destruct (decide (i = ι)).
-           * subst. by setoid_rewrite lookup_insert.
-           * setoid_rewrite lookup_insert_ne; auto.
-             setoid_rewrite lookup_insert_ne in HH; auto.
-         }
-         setoid_rewrite H0.
-         eapply n_other. econstructor.
-         by right; right; left.
+          apply map_eq. intros.
+          clear -H1.
+          put (lookup i : ProcessPool -> _) on H1 as HH.
+          destruct (decide (i = ι)).
+          * subst. by setoid_rewrite lookup_insert.
+          * setoid_rewrite lookup_insert_ne; auto.
+            setoid_rewrite lookup_insert_ne in HH; auto.
+        }
+        setoid_rewrite H0.
+        eapply n_other. eapply p_recv_peek_message_ok.
+        assumption.
+        by intuition.
       (* removeMessage *)
       + eexists. split.
         1: { constructor. eassumption. constructor. }
@@ -2807,7 +1395,115 @@ TODO: this cases a lot of boiler plate
        eapply n_other.
        econstructor.
        assumption.
-       by right; right; left.
+       by intuition.
+     (* recv_wait_timeout 0 *)
+      + eexists. split.
+        1: { constructor. eassumption. constructor. }
+        right.
+        assert (ι
+ ↦ inl
+     (FParams (IPrimOp "recv_wait_timeout") [] [] :: fs0, RValSeq [
+      VLit 0%Z], mb, ιs :: links, flag) ∥ prs = ι
+ ↦ inl
+     (FParams (IPrimOp "recv_wait_timeout") [] [] :: fs0, RValSeq [
+      VLit 0%Z], mb, ιs :: links, flag) ∥ Π). {
+          apply map_eq. intros.
+          clear -H1.
+          put (lookup i : ProcessPool -> _) on H1 as HH.
+          destruct (decide (i = ι)).
+          * subst. by setoid_rewrite lookup_insert.
+          * setoid_rewrite lookup_insert_ne; auto.
+            setoid_rewrite lookup_insert_ne in HH; auto.
+        }
+        setoid_rewrite H0.
+        eapply n_other. by constructor. by left.
+      (* recv_wait_timeout error *)
+      + eexists. split.
+        1: { constructor. eassumption. constructor. }
+        right.
+        assert (ι
+ ↦ inl
+     (FParams (IPrimOp "recv_wait_timeout") [] [] :: fs0, RValSeq [v], mb,
+      ιs :: links, flag) ∥ prs = ι
+ ↦ inl
+     (FParams (IPrimOp "recv_wait_timeout") [] [] :: fs0, RValSeq [v], mb,
+      ιs :: links, flag) ∥ Π). {
+          apply map_eq. intros.
+          clear -H1.
+          put (lookup i : ProcessPool -> _) on H1 as HH.
+          destruct (decide (i = ι)).
+          * subst. by setoid_rewrite lookup_insert.
+          * setoid_rewrite lookup_insert_ne; auto.
+            setoid_rewrite lookup_insert_ne in HH; auto.
+        }
+        setoid_rewrite H0.
+        eapply n_other. by constructor. by left.
+      (* self *)
+      + eexists. split.
+        1: { constructor. eassumption. constructor. }
+        right.
+        assert (ι
+ ↦ inl
+     (FParams (ICall (VLit "erlang"%string) (VLit "self"%string)) [] []
+      :: fs0, RBox, mb, ιs :: links, flag) ∥ prs = ι
+ ↦ inl
+     (FParams (ICall (VLit "erlang"%string) (VLit "self"%string)) [] []
+      :: fs0, RBox, mb, ιs :: links, flag) ∥ Π). {
+          apply map_eq. intros.
+          clear -H1.
+          put (lookup i : ProcessPool -> _) on H1 as HH.
+          destruct (decide (i = ι)).
+          * subst. by setoid_rewrite lookup_insert.
+          * setoid_rewrite lookup_insert_ne; auto.
+            setoid_rewrite lookup_insert_ne in HH; auto.
+        }
+        setoid_rewrite H0.
+        eapply n_other. by constructor. by right; left.
+      (* recv_peek_message - fail *)
+      + eexists. split.
+        1: { constructor. eassumption. constructor. }
+        right.
+        assert (ι
+ ↦ inl
+     (FParams (IPrimOp "recv_peek_message") [] [] :: fs0, RBox, mb,
+      ιs :: links, flag) ∥ prs = ι
+ ↦ inl
+     (FParams (IPrimOp "recv_peek_message") [] [] :: fs0, RBox, mb,
+      ιs :: links, flag) ∥ Π). {
+          apply map_eq. intros.
+          clear -H1.
+          put (lookup i : ProcessPool -> _) on H1 as HH.
+          destruct (decide (i = ι)).
+          * subst. by setoid_rewrite lookup_insert.
+          * setoid_rewrite lookup_insert_ne; auto.
+            setoid_rewrite lookup_insert_ne in HH; auto.
+        }
+        setoid_rewrite H0.
+        eapply n_other. econstructor.
+        assumption.
+        by intuition.
+      (* recv_next *)
+      + eexists. split.
+        1: { constructor. eassumption. constructor. }
+        right.
+        assert (ι
+ ↦ inl
+     (FParams (IPrimOp "recv_next") [] [] :: fs0, RBox, mb, 
+      ιs :: links, flag) ∥ prs = ι
+ ↦ inl
+     (FParams (IPrimOp "recv_next") [] [] :: fs0, RBox, mb, 
+      ιs :: links, flag) ∥ Π). {
+           apply map_eq. intros.
+           clear -H1.
+           put (lookup i : ProcessPool -> _) on H1 as HH.
+           destruct (decide (i = ι)).
+           * subst. by setoid_rewrite lookup_insert.
+           * setoid_rewrite lookup_insert_ne; auto.
+             setoid_rewrite lookup_insert_ne in HH; auto.
+         }
+         setoid_rewrite H0.
+         eapply n_other. econstructor.
+         by intuition.
       (* recv_wait_timeout infinity *)
       + eexists. split.
         1: { constructor. eassumption. constructor. }
@@ -2832,11 +1528,11 @@ TODO: this cases a lot of boiler plate
         setoid_rewrite H0.
         eapply n_other.
         econstructor.
-        by right; right; left.
+        by intuition.
       (* normal termination *)
-      + admit. (* arrive can't be chained on a dead process *)
+      + inv H. (* arrive can't be chained on a dead process *)
       (* exceptional termination *)
-      + admit. (* arrive can't be chained on a dead process *)
+      + inv H. (* arrive can't be chained on a dead process *)
       (* setflag *)
       + inv H.
     (* spawn *)
@@ -2913,16 +1609,16 @@ TODO: this cases a lot of boiler plate
  ↦ inl
      (FParams (ICall (VLit "erlang"%string) (VLit "!"%string)) [VPid ι'] []
       :: fs0, RValSeq [v], mb, remove numbers.Nat.eq_dec ιs links, flag) ∥ prs0). {
-               apply map_eq. intros.
-               clear -H2.
-               put (lookup i : ProcessPool -> _) on H2 as HH.
-               destruct (decide (i = ι)).
-               * subst. by setoid_rewrite lookup_insert.
-               * setoid_rewrite lookup_insert_ne; auto.
-                 setoid_rewrite lookup_insert_ne in HH; auto.
-             }
-             setoid_rewrite H0.
-             eapply n_send. by constructor.
+          apply map_eq. intros.
+          clear -H2.
+          put (lookup i : ProcessPool -> _) on H2 as HH.
+          destruct (decide (i = ι)).
+          * subst. by setoid_rewrite lookup_insert.
+          * setoid_rewrite lookup_insert_ne; auto.
+            setoid_rewrite lookup_insert_ne in HH; auto.
+        }
+        setoid_rewrite H0.
+        eapply n_send. by constructor.
       (* exit send *)
       + eexists. split.
         1: { constructor. apply etherPop_greater. eassumption.
@@ -2936,16 +1632,16 @@ TODO: this cases a lot of boiler plate
  ↦ inl
      (FParams (ICall (VLit "erlang"%string) (VLit "exit"%string)) [
         VPid ι'] [] :: fs0, RValSeq [v], mb, remove numbers.Nat.eq_dec ιs links, flag) ∥ prs0). {
-               apply map_eq. intros.
-               clear -H2.
-               put (lookup i : ProcessPool -> _) on H2 as HH.
-               destruct (decide (i = ι)).
-               * subst. by setoid_rewrite lookup_insert.
-               * setoid_rewrite lookup_insert_ne; auto.
-                 setoid_rewrite lookup_insert_ne in HH; auto.
-             }
-             setoid_rewrite H0.
-             eapply n_send. by constructor.
+          apply map_eq. intros.
+          clear -H2.
+          put (lookup i : ProcessPool -> _) on H2 as HH.
+          destruct (decide (i = ι)).
+          * subst. by setoid_rewrite lookup_insert.
+          * setoid_rewrite lookup_insert_ne; auto.
+            setoid_rewrite lookup_insert_ne in HH; auto.
+        }
+        setoid_rewrite H0.
+        eapply n_send. by constructor.
       (* link send - maybe this should not be proved? *)
       + eexists. split.
         1: { constructor. apply etherPop_greater. eassumption.
@@ -2959,18 +1655,18 @@ TODO: this cases a lot of boiler plate
  ↦ inl
      (FParams (ICall (VLit "erlang"%string) (VLit "link"%string)) [] []
       :: fs0, RValSeq [VPid ι'], mb, remove numbers.Nat.eq_dec ιs links, flag) ∥ prs0). {
-               apply map_eq. intros.
-               clear -H2.
-               put (lookup i : ProcessPool -> _) on H2 as HH.
-               destruct (decide (i = ι)).
-               * subst. by setoid_rewrite lookup_insert.
-               * setoid_rewrite lookup_insert_ne; auto.
-                 setoid_rewrite lookup_insert_ne in HH; auto.
-             }
-             setoid_rewrite H0.
-             eapply n_send. admit. (* TODO: links should be formalised as sets *)
+          apply map_eq. intros.
+          clear -H2.
+          put (lookup i : ProcessPool -> _) on H2 as HH.
+          destruct (decide (i = ι)).
+          * subst. by setoid_rewrite lookup_insert.
+          * setoid_rewrite lookup_insert_ne; auto.
+            setoid_rewrite lookup_insert_ne in HH; auto.
+        }
+        setoid_rewrite H0.
+        eapply n_send. inv H. (* TODO: links should be formalised as sets *)
       (* unlink send - can't be proved if the same link is established and deleted in the two reductions *)
-      + admit.
+      + inv H.
     (* arrivals - cannot happen *)
     - inv H.
     (* local actions *)
@@ -2988,79 +1684,16 @@ TODO: this cases a lot of boiler plate
         1: { constructor. eassumption. constructor. }
         right.
         assert (ι ↦ inl (fs, e, mb, remove numbers.Nat.eq_dec ιs links, flag) ∥ prs = ι ↦ inl (fs, e, mb, remove numbers.Nat.eq_dec ιs links, flag) ∥ Π). {
-               apply map_eq. intros.
-               clear -H1.
-               put (lookup i : ProcessPool -> _) on H1 as HH.
-               destruct (decide (i = ι)).
-               * subst. by setoid_rewrite lookup_insert.
-               * setoid_rewrite lookup_insert_ne; auto.
-                 setoid_rewrite lookup_insert_ne in HH; auto.
-             }
-             setoid_rewrite H0.
-             eapply n_other. by constructor. by left.
-      (* recv_wait_timeout 0 *)
-      + eexists. split.
-        1: { constructor. eassumption. constructor. }
-        right.
-        assert (ι
- ↦ inl
-     (FParams (IPrimOp "recv_wait_timeout") [] [] :: fs0, RValSeq [
-      VLit 0%Z], mb, remove numbers.Nat.eq_dec ιs links, flag) ∥ prs = ι
- ↦ inl
-     (FParams (IPrimOp "recv_wait_timeout") [] [] :: fs0, RValSeq [
-      VLit 0%Z], mb, remove numbers.Nat.eq_dec ιs links, flag) ∥ Π). {
-               apply map_eq. intros.
-               clear -H1.
-               put (lookup i : ProcessPool -> _) on H1 as HH.
-               destruct (decide (i = ι)).
-               * subst. by setoid_rewrite lookup_insert.
-               * setoid_rewrite lookup_insert_ne; auto.
-                 setoid_rewrite lookup_insert_ne in HH; auto.
-             }
-             setoid_rewrite H0.
-             eapply n_other. by constructor. by left.
-      (* recv_wait_timeout error *)
-      + eexists. split.
-        1: { constructor. eassumption. constructor. }
-        right.
-        assert (ι
- ↦ inl
-     (FParams (IPrimOp "recv_wait_timeout") [] [] :: fs0, RValSeq [v], mb,
-      remove numbers.Nat.eq_dec ιs links, flag) ∥ prs = ι
- ↦ inl
-     (FParams (IPrimOp "recv_wait_timeout") [] [] :: fs0, RValSeq [v], mb,
-      remove numbers.Nat.eq_dec ιs links, flag) ∥ Π). {
-               apply map_eq. intros.
-               clear -H1.
-               put (lookup i : ProcessPool -> _) on H1 as HH.
-               destruct (decide (i = ι)).
-               * subst. by setoid_rewrite lookup_insert.
-               * setoid_rewrite lookup_insert_ne; auto.
-                 setoid_rewrite lookup_insert_ne in HH; auto.
-             }
-             setoid_rewrite H0.
-             eapply n_other. by constructor. by left.
-      (* self *)
-      + eexists. split.
-        1: { constructor. eassumption. constructor. }
-        right.
-        assert (ι
- ↦ inl
-     (FParams (ICall (VLit "erlang"%string) (VLit "self"%string)) [] []
-      :: fs0, RBox, mb, remove numbers.Nat.eq_dec ιs links, flag) ∥ prs = ι
- ↦ inl
-     (FParams (ICall (VLit "erlang"%string) (VLit "self"%string)) [] []
-      :: fs0, RBox, mb, remove numbers.Nat.eq_dec ιs links, flag) ∥ Π). {
-               apply map_eq. intros.
-               clear -H1.
-               put (lookup i : ProcessPool -> _) on H1 as HH.
-               destruct (decide (i = ι)).
-               * subst. by setoid_rewrite lookup_insert.
-               * setoid_rewrite lookup_insert_ne; auto.
-                 setoid_rewrite lookup_insert_ne in HH; auto.
-             }
-             setoid_rewrite H0.
-             eapply n_other. by constructor. by right; left.
+          apply map_eq. intros.
+          clear -H1.
+          put (lookup i : ProcessPool -> _) on H1 as HH.
+          destruct (decide (i = ι)).
+          * subst. by setoid_rewrite lookup_insert.
+          * setoid_rewrite lookup_insert_ne; auto.
+            setoid_rewrite lookup_insert_ne in HH; auto.
+        }
+        setoid_rewrite H0.
+        eapply n_other. by constructor. by left.
       (* recv_peek_message - success *)
       + eexists. split.
         1: { constructor. eassumption. constructor. }
@@ -3072,63 +1705,18 @@ TODO: this cases a lot of boiler plate
  ↦ inl
      (FParams (IPrimOp "recv_peek_message") [] [] :: fs0, RBox, mb,
       remove numbers.Nat.eq_dec ιs links, flag) ∥ Π). {
-               apply map_eq. intros.
-               clear -H1.
-               put (lookup i : ProcessPool -> _) on H1 as HH.
-               destruct (decide (i = ι)).
-               * subst. by setoid_rewrite lookup_insert.
-               * setoid_rewrite lookup_insert_ne; auto.
-                 setoid_rewrite lookup_insert_ne in HH; auto.
-             }
-             setoid_rewrite H0.
-             eapply n_other. econstructor.
-             assumption.
-             by right; right; left.
-      (* recv_peek_message - fail *)
-      + eexists. split.
-        1: { constructor. eassumption. constructor. }
-        right.
-        assert (ι
- ↦ inl
-     (FParams (IPrimOp "recv_peek_message") [] [] :: fs0, RBox, mb,
-      remove numbers.Nat.eq_dec ιs links, flag) ∥ prs = ι
- ↦ inl
-     (FParams (IPrimOp "recv_peek_message") [] [] :: fs0, RBox, mb,
-      remove numbers.Nat.eq_dec ιs links, flag) ∥ Π). {
-               apply map_eq. intros.
-               clear -H1.
-               put (lookup i : ProcessPool -> _) on H1 as HH.
-               destruct (decide (i = ι)).
-               * subst. by setoid_rewrite lookup_insert.
-               * setoid_rewrite lookup_insert_ne; auto.
-                 setoid_rewrite lookup_insert_ne in HH; auto.
-             }
-             setoid_rewrite H0.
-             eapply n_other. econstructor.
-             assumption.
-             by right; right; left.
-      (* recv_next *)
-      + eexists. split.
-        1: { constructor. eassumption. constructor. }
-        right.
-        assert (ι
- ↦ inl
-     (FParams (IPrimOp "recv_next") [] [] :: fs0, RBox, mb, 
-      remove numbers.Nat.eq_dec ιs links, flag) ∥ prs = ι
- ↦ inl
-     (FParams (IPrimOp "recv_next") [] [] :: fs0, RBox, mb, 
-      remove numbers.Nat.eq_dec ιs links, flag) ∥ Π). {
-           apply map_eq. intros.
-           clear -H1.
-           put (lookup i : ProcessPool -> _) on H1 as HH.
-           destruct (decide (i = ι)).
-           * subst. by setoid_rewrite lookup_insert.
-           * setoid_rewrite lookup_insert_ne; auto.
-             setoid_rewrite lookup_insert_ne in HH; auto.
-         }
-         setoid_rewrite H0.
-         eapply n_other. econstructor.
-         by right; right; left.
+          apply map_eq. intros.
+          clear -H1.
+          put (lookup i : ProcessPool -> _) on H1 as HH.
+          destruct (decide (i = ι)).
+          * subst. by setoid_rewrite lookup_insert.
+          * setoid_rewrite lookup_insert_ne; auto.
+            setoid_rewrite lookup_insert_ne in HH; auto.
+        }
+        setoid_rewrite H0.
+        eapply n_other. eapply p_recv_peek_message_ok.
+        assumption.
+        by intuition.
       (* removeMessage *)
       + eexists. split.
         1: { constructor. eassumption. constructor. }
@@ -3152,7 +1740,115 @@ TODO: this cases a lot of boiler plate
        eapply n_other.
        econstructor.
        assumption.
-       by right; right; left.
+       by intuition.
+      (* recv_wait_timeout 0 *)
+      + eexists. split.
+        1: { constructor. eassumption. constructor. }
+        right.
+        assert (ι
+ ↦ inl
+     (FParams (IPrimOp "recv_wait_timeout") [] [] :: fs0, RValSeq [
+      VLit 0%Z], mb, remove numbers.Nat.eq_dec ιs links, flag) ∥ prs = ι
+ ↦ inl
+     (FParams (IPrimOp "recv_wait_timeout") [] [] :: fs0, RValSeq [
+      VLit 0%Z], mb, remove numbers.Nat.eq_dec ιs links, flag) ∥ Π). {
+          apply map_eq. intros.
+          clear -H1.
+          put (lookup i : ProcessPool -> _) on H1 as HH.
+          destruct (decide (i = ι)).
+          * subst. by setoid_rewrite lookup_insert.
+          * setoid_rewrite lookup_insert_ne; auto.
+            setoid_rewrite lookup_insert_ne in HH; auto.
+        }
+        setoid_rewrite H0.
+        eapply n_other. by constructor. by left.
+      (* recv_wait_timeout error *)
+      + eexists. split.
+        1: { constructor. eassumption. constructor. }
+        right.
+        assert (ι
+ ↦ inl
+     (FParams (IPrimOp "recv_wait_timeout") [] [] :: fs0, RValSeq [v], mb,
+      remove numbers.Nat.eq_dec ιs links, flag) ∥ prs = ι
+ ↦ inl
+     (FParams (IPrimOp "recv_wait_timeout") [] [] :: fs0, RValSeq [v], mb,
+      remove numbers.Nat.eq_dec ιs links, flag) ∥ Π). {
+          apply map_eq. intros.
+          clear -H1.
+          put (lookup i : ProcessPool -> _) on H1 as HH.
+          destruct (decide (i = ι)).
+          * subst. by setoid_rewrite lookup_insert.
+          * setoid_rewrite lookup_insert_ne; auto.
+            setoid_rewrite lookup_insert_ne in HH; auto.
+        }
+        setoid_rewrite H0.
+        eapply n_other. by constructor. by left.
+      (* self *)
+      + eexists. split.
+        1: { constructor. eassumption. constructor. }
+        right.
+        assert (ι
+ ↦ inl
+     (FParams (ICall (VLit "erlang"%string) (VLit "self"%string)) [] []
+      :: fs0, RBox, mb, remove numbers.Nat.eq_dec ιs links, flag) ∥ prs = ι
+ ↦ inl
+     (FParams (ICall (VLit "erlang"%string) (VLit "self"%string)) [] []
+      :: fs0, RBox, mb, remove numbers.Nat.eq_dec ιs links, flag) ∥ Π). {
+          apply map_eq. intros.
+          clear -H1.
+          put (lookup i : ProcessPool -> _) on H1 as HH.
+          destruct (decide (i = ι)).
+          * subst. by setoid_rewrite lookup_insert.
+          * setoid_rewrite lookup_insert_ne; auto.
+            setoid_rewrite lookup_insert_ne in HH; auto.
+        }
+        setoid_rewrite H0.
+        eapply n_other. by constructor. by right; left.
+      (* recv_peek_message - fail *)
+      + eexists. split.
+        1: { constructor. eassumption. constructor. }
+        right.
+        assert (ι
+ ↦ inl
+     (FParams (IPrimOp "recv_peek_message") [] [] :: fs0, RBox, mb,
+      remove numbers.Nat.eq_dec ιs links, flag) ∥ prs = ι
+ ↦ inl
+     (FParams (IPrimOp "recv_peek_message") [] [] :: fs0, RBox, mb,
+      remove numbers.Nat.eq_dec ιs links, flag) ∥ Π). {
+          apply map_eq. intros.
+          clear -H1.
+          put (lookup i : ProcessPool -> _) on H1 as HH.
+          destruct (decide (i = ι)).
+          * subst. by setoid_rewrite lookup_insert.
+          * setoid_rewrite lookup_insert_ne; auto.
+            setoid_rewrite lookup_insert_ne in HH; auto.
+        }
+        setoid_rewrite H0.
+        eapply n_other. econstructor.
+        assumption.
+        by intuition.
+      (* recv_next *)
+      + eexists. split.
+        1: { constructor. eassumption. constructor. }
+        right.
+        assert (ι
+ ↦ inl
+     (FParams (IPrimOp "recv_next") [] [] :: fs0, RBox, mb, 
+      remove numbers.Nat.eq_dec ιs links, flag) ∥ prs = ι
+ ↦ inl
+     (FParams (IPrimOp "recv_next") [] [] :: fs0, RBox, mb, 
+      remove numbers.Nat.eq_dec ιs links, flag) ∥ Π). {
+           apply map_eq. intros.
+           clear -H1.
+           put (lookup i : ProcessPool -> _) on H1 as HH.
+           destruct (decide (i = ι)).
+           * subst. by setoid_rewrite lookup_insert.
+           * setoid_rewrite lookup_insert_ne; auto.
+             setoid_rewrite lookup_insert_ne in HH; auto.
+         }
+         setoid_rewrite H0.
+         eapply n_other. econstructor.
+         by intuition.
       (* recv_wait_timeout infinity *)
       + eexists. split.
         1: { constructor. eassumption. constructor. }
@@ -3177,11 +1873,11 @@ TODO: this cases a lot of boiler plate
         setoid_rewrite H0.
         eapply n_other.
         econstructor.
-        by right; right; left.
+        by intuition.
       (* normal termination *)
-      + admit. (* arrive can't be chained on a dead process *)
+      + inv H. (* arrive can't be chained on a dead process *)
       (* exceptional termination *)
-      + admit. (* arrive can't be chained on a dead process *)
+      + inv H. (* arrive can't be chained on a dead process *)
       (* setflag *)
       + inv H.
     (* spawn *)
@@ -3236,8 +1932,47 @@ TODO: this cases a lot of boiler plate
         intro. eapply appearsEther_etherPop_rev in H; eauto.
       }
       constructor; assumption.
-Admitted.
+Qed.
 
+Check chain_arrive_later.
+(*
+  THOUGHTS.
+  We can't prove normalisation of "Playing with bisimulation in Erlang".
+  We could prove normalisation up to exits in a fully general way (spawns,
+  compatible sends and τ could be included in the normalisation chain), though.
+
+  Although, currently we couldn't prove map and concurrent map equivalent for
+  their naive implementations?
+  - The issue is with exit arriving after/before doing a spawn:
+    - Parent terminates:
+        One process will compute the result of the map, then send this result
+        to the terminated parent, then it terminates. Since the parent is not
+        in O (it is not observed), this would not show up in the observed messages.
+    - Child terminates:
+        Parent will be waiting forever for a message from the child
+
+  To rule out exits, we can use the following approaches:
+  - Define barbed bisimulation up to exits (~ᵉ), and prove that:
+      A ~ B -> A ~ᵉ B
+  - Is it enough to ensure that in the starting configuration, there are no
+    exits in the ether? I suppose not, because the system can introduce them
+    during evaluation, and we do not know how/when they get delivered.
+  - No exits in the ether, and the reductions should not send exits.
+  - We do not rule out exits from the normalisation, but then we have to rule out
+    spawns.
+
+  Would some mechanism (e.g., spawn_link), which would give us guarantees that
+  the spawned process will be terminated too?
+  - In this case, confluence is not going to be strict obviously
+
+  What if instead of an ether, we use an individual ether for each process,
+  and the process local semantics determines whether it moves something from
+  there to the mailbox/terminates the process/drops signals, etc.?
+  - Probably would not help, since there should be an action representing
+    this step of the local semantics which should be confluent with the others.
+
+
+*)
 Theorem action_chainable :
   (* NOTE: only l (and n n') can be constrained for the proof of normalisation!
      NOTE: don't forget that 
@@ -3940,161 +2675,15 @@ Proof.
     }
 Abort.
 
-Theorem arrive_chain :
-  forall O A B C a ι s ιs,
-    A -[a|ι]ₙ-> B with O ->
-    A -[AArrive ιs ι s|ι]ₙ-> C with O ->
-    (a = AArrive ιs ι s) \/
-    (exists D, B -[AArrive ιs ι s| ι]ₙ-> D with O) \/
-    (B = (A.1, C.2)) (* One of the actions can't happen due to termination *).
-Proof.
-  intros. inv H; inv H0; subst.
-  * 
-  *
-  *
-  *
-  *
-  *
-  *
-  *
-Qed.
+(* This would be a consequence of normalisation, but exits break this property
+   too. E.g., a potential exit could terminate A, and not B. *)
+Theorem normalise_common :
+  forall A B C O l₁ l₂,
+    A -[l₁]ₙ->* C with O ->
+    B -[l₂]ₙ->* C with O ->
+    A ~ B observing O.
 
 
 
 
-
-
-
-Lemma bisim_congr :
-  forall U Π Π' eth eth', (eth, Π) ~ (eth', Π') using U ->
-    forall Π2, (eth, Π ∪ Π2) ~ (eth', Π' ∪ Π2) using U.
-Proof.
-  cofix IH. intros. inv H. constructor; auto; simpl in *.
-  * clear -H0. destruct H0. split; unfold preCompatibleNodes in *; intros.
-    - apply isUntaken_comp in H1 as [H1_1 H1_2].
-      apply H in H1_1.
-      assert (isUntaken ι (eth', Π2)). {
-        destruct H1_1, H1_2. split; auto.
-      }
-      now apply isUntaken_comp.
-    - apply isUntaken_comp in H1 as [H1_1 H1_2].
-      apply H0 in H1_1.
-      assert (isUntaken ι (eth, Π2)). {
-        destruct H1_1, H1_2. split; auto.
-      }
-      now apply isUntaken_comp.
-  * clear H4 H5 H6. intros. destruct A'.
-    apply step_in_comp in H as H'. destruct H' as [[Π1' [? ?]] | [Π2' [? ?]]].
-    - subst. apply H3 in H4 as H4'. destruct_hyps. destruct x as [e' Π1''].
-      (* (* At this point, we need renamings :( - or to know what PIDs are
-         spawned by Π *)
-      Print reductionPreCompatibility.
-      (* spawns in x0 should be distinct from:
-         - syntactically used PIDs in Π2 - for goal 3
-         - ι0 -> if a = send(ι, ι0 <- destination, msg)
-         - We also need a proof that (eth, Π) ~ (eth[x|->y], Π[x|->y])
-      *)
-      exists (e', Π1'' ∪ Π2), x0. split. 2: split. 3: split.
-      4: { apply IH. assumption. }
-      3: apply reductions_are_preserved_by_comp; auto.
-      3: {
-        intros. destruct H6 as [H6 _]. rewrite Forall_forall in H6.
-        apply H6 in H9. unfold isUntaken in H9. simpl in *.
-      } *)
-      admit.
-    - subst. exists (e, Π' ∪ Π2'), [(a, ι)]. split_and!.
-      + split.
-        ** destruct a; auto. simpl. constructor; auto. intro.
-           eapply (no_spawn_unTaken (eth, Π ∪ Π2)). eapply n_trans. eassumption.
-           apply n_refl. 2: cbn; left; reflexivity.
-           apply isUntaken_comp in H5 as [? ?]. apply H0 in H5.
-           apply isUntaken_comp; split; auto.
-           (* ι0 should be Untaken wrt. eth *)
-           destruct H5, H6. split; simpl in *; auto.
-        ** intros; simpl in *; destruct a; auto; simpl in *.
-           destruct_or!; auto. split. 2: split; auto.
-           subst.
-           (* ISSUE: we do not know, whether Π' uses ι0 *)
-           (* is it okay to assume, that Π2 does not communicate to 
-              PIDs in the domain of Π/Π' -> NO!
-
-              is it okay to assume, that Π2 does not communicate to
-              PIDs in ((dom Π ∪ dom Π') \ (dom Π ∩ dom Π')). Probably not.
-            *)
-           admit.
-      + split.
-        ** destruct a; auto. simpl. constructor; auto. intro.
-           eapply (no_spawn_unTaken (eth, Π ∪ Π2)). eapply n_trans. eassumption.
-           apply n_refl. 2: cbn; left; reflexivity.
-           apply isUntaken_comp in H5 as [? ?].
-           apply isUntaken_comp; split; auto.
-        ** intros; simpl in *; destruct a; auto; simpl in *.
-           destruct_or!; auto. split. 2: split; auto.
-           subst.
-           (* ISSUE: we do not know, whether Π uses ι0
-              BOTTOMLINE: we should specify where can Π2 send messages?
-            *)
-           admit.
-      + econstructor.
-        apply reduction_is_preserved_by_comp_r. (* eassumption. *) admit. admit. admit. admit.
-      + admit.
-(*     - subst. exists (e, Π ∪ Π2'), [(a, ι)]. split_and!.
-      split.
-      + destruct a; auto. simpl. constructor; auto. intro.
-        eapply (no_spawn_unTaken (eth, Π ∪ Π2)). eapply n_trans. eassumption.
-        apply n_refl. 2: cbn; left; reflexivity.
-        apply isUntaken_comp in H5 as [? ?]. apply H0 in H5.
-        apply isUntaken_comp; split; auto.
-        (* ι0 should be Untaken wrt. eth *)
-        destruct H5, H6. split; simpl in *; auto.
-      + intros; simpl in *; destruct a; auto; simpl in *.
-        destruct_or!; auto. split. 2: split; auto.
-        subst.
-        (* ISSUE: we do not know, whether Π' uses ι0 *)
-        admit.
-      4: { apply IH. apply barbedBisim_refl. } *)
-Abort.
-
-
-
-
-
-
-
-
-
-
-
-
-
-
-
-
-Theorem action_chainable:
-  forall l n n', n -[l]ₙ->* n' ->
-    (* (forall ι : PID, In ι (PIDsOf sendPIDOf l) -> n'.2 ι <> None) -> *)
-    (* (forall ι ι' : PID, n.2 ι' = None -> n.1 ι ι' = []) -> *)
-    forall a ι n'', n -[a | ι]ₙ-> n'' ->
-      In (a, ι) l \/ 
-      exists n''' a' ι', n' -[a' | ι']ₙ-> n''' /\
-               reductionPreCompatibility n n' [(a, ι)] [(a', ι')] /\
-               reductionPreCompatibility n' n [(a', ι')] [(a, ι)].
-Proof.
-  induction l using list_length_ind; intros.
-  
-  (* induction l using list_length_ind; intros.
-  destruct (length l) eqn:Hl.
-  * apply length_zero_iff_nil in Hl. subst.
-    inv H0. right. exists n'', a, ι.
-    split; auto.
-    split; eapply reductionPreCompatibility_refl; eassumption.
-  * simpl in Hl. apply eq_sym, last_element_exists in Hl as Hl'.
-    destruct Hl' as [l' [[a' ι'] EQ]]. subst.
-    apply split_reduction in H0 as [n'0 [D1 D2]].
-    rewrite app_length in Hl. simpl in Hl.
-    specialize (H l' ltac:(lia) _ _ D1 _ _ _ H1). destruct H.
-    - left. apply elem_of_app. now left.
-    - rename n'0 into A. rename n' into B.
-      destruct_hyps. inv D2. inv H9. *)
-Abort.
 
